@prefix : <https://github.com/UTEP-Dynamic-Materials-Lab/SHPB_Toolkit/tree/main/ontology#> .
@prefix owl: <http://www.w3.org/2002/07/owl#> .
@prefix rdf: <http://www.w3.org/1999/02/22-rdf-syntax-ns#> .
@prefix xml: <http://www.w3.org/XML/1998/namespace> .
@prefix xsd: <http://www.w3.org/2001/XMLSchema#> .
@prefix rdfs: <http://www.w3.org/2000/01/rdf-schema#> .
@base <https://github.com/UTEP-Dynamic-Materials-Lab/SHPB_Toolkit/tree/main/ontology#> .

<https://github.com/UTEP-Dynamic-Materials-Lab/SHPB_Toolkit/tree/main/ontology> rdf:type owl:Ontology .

#################################################################
#    Annotation properties
#################################################################

###  https://github.com/UTEP-Dynamic-Materials-Lab/SHPB_Toolkit/tree/main/ontology#hasAfilliation
:hasAfilliation rdf:type owl:AnnotationProperty .


###  https://github.com/UTEP-Dynamic-Materials-Lab/SHPB_Toolkit/tree/main/ontology#hasMaterialType
:hasMaterialType rdf:type owl:AnnotationProperty .


###  https://github.com/UTEP-Dynamic-Materials-Lab/SHPB_Toolkit/tree/main/ontology#hasName
:hasName rdf:type owl:AnnotationProperty ;
         rdfs:range xsd:string .


#################################################################
#    Datatypes
#################################################################

###  http://www.w3.org/2001/XMLSchema#date
xsd:date rdf:type rdfs:Datatype .


#################################################################
#    Object Properties
#################################################################

###  https://github.com/UTEP-Dynamic-Materials-Lab/SHPB_Toolkit/tree/main/ontology#hasBar
:hasBar rdf:type owl:ObjectProperty ;
        rdfs:domain :TestingConditions ;
        rdfs:range :Bar ;
        rdfs:comment "Used to relate SHPB testing conditions to a defined instance of the Bar Class" .


###  https://github.com/UTEP-Dynamic-Materials-Lab/SHPB_Toolkit/tree/main/ontology#hasDimension
:hasDimension rdf:type owl:ObjectProperty ;
              rdfs:subPropertyOf owl:topObjectProperty ;
              rdfs:domain :Bar ,
                          :Specimen ;
              rdfs:range :Dimension ;
              rdfs:comment "Relates a Specimen or Bar to their measurable physical Dimension" .


###  https://github.com/UTEP-Dynamic-Materials-Lab/SHPB_Toolkit/tree/main/ontology#hasExtractedSignal
:hasExtractedSignal rdf:type owl:ObjectProperty ;
                    rdfs:domain :SecondaryData ;
                    rdfs:range :ExtractedSignal ;
                    rdfs:comment "Assigns Secondary Data extracted SHPB signals used later in post-process analysis" .


###  https://github.com/UTEP-Dynamic-Materials-Lab/SHPB_Toolkit/tree/main/ontology#hasFEAMetadata
:hasFEAMetadata rdf:type owl:ObjectProperty ;
                rdfs:subPropertyOf owl:topObjectProperty ;
                rdfs:domain [ rdf:type owl:Class ;
                              owl:unionOf ( :Bar
                                            :Specimen
                                          )
                            ] ;
                rdfs:range :FEAMetadata ;
                rdfs:comment "Relates a Bar or Specimen instance to its FEA metadata, which describes the object in a FE model." .


###  https://github.com/UTEP-Dynamic-Materials-Lab/SHPB_Toolkit/tree/main/ontology#hasFiniteElement
:hasFiniteElement rdf:type owl:ObjectProperty ;
                  rdfs:domain :FEAMetadata ,
                              :FiniteElement ;
                  rdfs:range :FiniteElement ;
                  rdfs:comment "Relates the FEA Metadata to a instance of a Finite Element that describes the object in a FEA Model" .


###  https://github.com/UTEP-Dynamic-Materials-Lab/SHPB_Toolkit/tree/main/ontology#hasLaboratory
:hasLaboratory rdf:type owl:ObjectProperty ;
               rdfs:domain :Metadata ;
               rdfs:range :Laboratory ;
               rdfs:comment "Relates Metadata to the Laboratory where experiments took place." .


###  https://github.com/UTEP-Dynamic-Materials-Lab/SHPB_Toolkit/tree/main/ontology#hasMaterial
:hasMaterial rdf:type owl:ObjectProperty ;
             rdfs:subPropertyOf owl:topObjectProperty ;
             rdfs:domain :Bar ,
                         :Specimen ;
             rdfs:range :Material ;
             rdfs:comment "Relates test specimens and testing conditions objects to their respective engineering Material" .


###  https://github.com/UTEP-Dynamic-Materials-Lab/SHPB_Toolkit/tree/main/ontology#hasMaterialHeatTreatment
:hasMaterialHeatTreatment rdf:type owl:ObjectProperty ;
                          rdfs:domain :Material .


###  https://github.com/UTEP-Dynamic-Materials-Lab/SHPB_Toolkit/tree/main/ontology#hasMechanicalProperty
:hasMechanicalProperty rdf:type owl:ObjectProperty ;
                       rdfs:domain :Bar ,
                                   :Specimen ;
                       rdfs:range :MechanicalProperty ;
                       rdfs:comment "Links a determined mechanical property from an experiment to the specimen." ,
                                    "Links a general mechanical property to a Bar or Specimen." .


###  https://github.com/UTEP-Dynamic-Materials-Lab/SHPB_Toolkit/tree/main/ontology#hasMetadata
:hasMetadata rdf:type owl:ObjectProperty ;
             rdfs:domain :Experiment ;
             rdfs:range :Metadata ;
             rdfs:comment "Links the Experiment instance to their Metadata entries" .


###  https://github.com/UTEP-Dynamic-Materials-Lab/SHPB_Toolkit/tree/main/ontology#hasMomentumTrap
:hasMomentumTrap rdf:type owl:ObjectProperty ;
                 rdfs:domain :TestingConditions ;
                 rdfs:range :MomentumTrap ;
                 rdfs:comment "Links metadata to test configurations of momentum trap engagement. Used in SHPB analysis" .


###  https://github.com/UTEP-Dynamic-Materials-Lab/SHPB_Toolkit/tree/main/ontology#hasParameter
:hasParameter rdf:type owl:ObjectProperty ;
              rdfs:domain :StrengthModel ;
              rdfs:range :MechanicalProperty ;
              rdfs:comment "Links a strength model to its parameters. Which are also Mechanical Properties." .


###  https://github.com/UTEP-Dynamic-Materials-Lab/SHPB_Toolkit/tree/main/ontology#hasPrimaryData
:hasPrimaryData rdf:type owl:ObjectProperty ;
                rdfs:domain :Experiment ;
                rdfs:range :PrimaryData ;
                rdfs:comment "Links the Experiment to its Primary Data entries" .


###  https://github.com/UTEP-Dynamic-Materials-Lab/SHPB_Toolkit/tree/main/ontology#hasPulseProperty
:hasPulseProperty rdf:type owl:ObjectProperty ;
                  rdfs:domain :SecondaryData ;
                  rdfs:range :PulseProperties ;
                  rdfs:comment "Links determined Pulse Properties of a SHPB experiment under Secondary Data" .


###  https://github.com/UTEP-Dynamic-Materials-Lab/SHPB_Toolkit/tree/main/ontology#hasSecondaryData
:hasSecondaryData rdf:type owl:ObjectProperty ;
                  rdfs:domain :Experiment ;
                  rdfs:range :SecondaryData ;
                  rdfs:comment "Links Experiments to their Secondary Data entries" .


###  https://github.com/UTEP-Dynamic-Materials-Lab/SHPB_Toolkit/tree/main/ontology#hasSensorSignal
:hasSensorSignal rdf:type owl:ObjectProperty ;
                 rdfs:domain :PrimaryData ;
                 rdfs:range :SensorSignal ;
                 rdfs:comment "Links primary data to specific sensor signals obtained during testing procedures." .


###  https://github.com/UTEP-Dynamic-Materials-Lab/SHPB_Toolkit/tree/main/ontology#hasSeriesData
:hasSeriesData rdf:type owl:ObjectProperty ;
               rdfs:domain :SecondaryData ;
               rdfs:range :SeriesData ;
               rdfs:comment "Links determined data Series Data, like stress and strain to the experiment's Secondary Data" .


###  https://github.com/UTEP-Dynamic-Materials-Lab/SHPB_Toolkit/tree/main/ontology#hasShape
:hasShape rdf:type owl:ObjectProperty ;
          rdfs:domain :Specimen ;
          rdfs:range :Shape ;
          rdfs:comment "Links the Specimen to their respective Shape" .


###  https://github.com/UTEP-Dynamic-Materials-Lab/SHPB_Toolkit/tree/main/ontology#hasSpecimen
:hasSpecimen rdf:type owl:ObjectProperty ;
             rdfs:domain :Metadata ;
             rdfs:range :Specimen ;
             rdfs:comment "Links Metadata to the Specimen details." .


###  https://github.com/UTEP-Dynamic-Materials-Lab/SHPB_Toolkit/tree/main/ontology#hasSpecimenProcessing
:hasSpecimenProcessing rdf:type owl:ObjectProperty ;
                       rdfs:subPropertyOf owl:topObjectProperty ;
                       rdfs:domain :Specimen ;
                       rdfs:range :SpecimenProcessing ;
                       rdfs:comment "Relates a Material to its Material Processing description" .


###  https://github.com/UTEP-Dynamic-Materials-Lab/SHPB_Toolkit/tree/main/ontology#hasStrainGauge
:hasStrainGauge rdf:type owl:ObjectProperty ;
                rdfs:subPropertyOf owl:topObjectProperty ;
                rdfs:domain :Bar ,
                            :SensorSignal ;
                rdfs:range :StrainGauge ;
                rdfs:comment "Links raw sensor signals to the respective gauge that captured that data. In SHPB analysis this is also included in the bars for post-process operations" .


###  https://github.com/UTEP-Dynamic-Materials-Lab/SHPB_Toolkit/tree/main/ontology#hasStrainGaugeProperty
:hasStrainGaugeProperty rdf:type owl:ObjectProperty ;
                        rdfs:domain :StrainGauge ;
                        rdfs:range :StrainGaugeProperties ;
                        rdfs:comment "Links laboratory strain gauges to strain gauge properties. Utilized in SHPB analysis to transform voltage to strain readings" .


###  https://github.com/UTEP-Dynamic-Materials-Lab/SHPB_Toolkit/tree/main/ontology#hasStrengthModel
:hasStrengthModel rdf:type owl:ObjectProperty ;
                  rdfs:domain :FEAMetadata ;
                  rdfs:range :StrengthModel ;
                  rdfs:comment "Links FEA Metadata to the associated Strength Model used for analysis." .


###  https://github.com/UTEP-Dynamic-Materials-Lab/SHPB_Toolkit/tree/main/ontology#hasStructure
:hasStructure rdf:type owl:ObjectProperty ;
              rdfs:subPropertyOf owl:topObjectProperty ;
              rdfs:domain :Specimen ;
              rdfs:range :Structure ;
              rdfs:comment "Links the Specimen to its defined Structure" .


###  https://github.com/UTEP-Dynamic-Materials-Lab/SHPB_Toolkit/tree/main/ontology#hasTestMode
:hasTestMode rdf:type owl:ObjectProperty ;
             rdfs:domain :TestingConditions ;
             rdfs:range :TestMode ;
             rdfs:comment "Links Testing Conditions to the Test Mode, which describes the physical or virtual conditions of the test." .


###  https://github.com/UTEP-Dynamic-Materials-Lab/SHPB_Toolkit/tree/main/ontology#hasTestTemperature
:hasTestTemperature rdf:type owl:ObjectProperty ;
                    rdfs:domain :TestingConditions ;
                    rdfs:range :TestTemperature ;
                    rdfs:comment "Links Testing Conditions with the Test Temperature used in the experiment" .


###  https://github.com/UTEP-Dynamic-Materials-Lab/SHPB_Toolkit/tree/main/ontology#hasTestType
:hasTestType rdf:type owl:ObjectProperty ;
             rdfs:domain :TestingConditions ;
             rdfs:range :TestType ;
             rdfs:comment "Links Testing Conditions to their test Type. Used to identify calibration from actual specimen experiments. Defines post-process analysis." .


###  https://github.com/UTEP-Dynamic-Materials-Lab/SHPB_Toolkit/tree/main/ontology#hasTestingConditions
:hasTestingConditions rdf:type owl:ObjectProperty ;
                      rdfs:domain :Metadata ;
                      rdfs:range :TestingConditions ;
                      rdfs:comment "Links Metadata to the Testing Conditions used to perform an experiment, such as lab-based or simulation-based." .


###  https://github.com/UTEP-Dynamic-Materials-Lab/SHPB_Toolkit/tree/main/ontology#hasUnits
:hasUnits rdf:type owl:ObjectProperty ;
          rdfs:domain :Dimension ,
                      :ExtractedSignal ,
                      :MechanicalProperty ,
                      :SensorSignal ,
                      :SeriesData ,
                      :StrainGaugeProperties ;
          rdfs:range :Unit ;
          rdfs:comment "Links a Dimension or Mechanical Property to its allowable units." .


###  https://github.com/UTEP-Dynamic-Materials-Lab/SHPB_Toolkit/tree/main/ontology#hasUser
:hasUser rdf:type owl:ObjectProperty ;
         rdfs:domain :TestingConditions ;
         rdfs:range :User ;
         rdfs:comment "Links Metadata to a User instance in charge of performing the experiment" .


#################################################################
#    Data properties
#################################################################

###  https://github.com/UTEP-Dynamic-Materials-Lab/SHPB_Toolkit/tree/main/ontology#hasAbbreviation
:hasAbbreviation rdf:type owl:DatatypeProperty ;
                 rdfs:domain [ rdf:type owl:Restriction ;
                               owl:onProperty :hasAbbreviation ;
                               owl:someValuesFrom xsd:string
                             ] ;
                 rdfs:comment "Abbreviation or initials of the user." .


###  https://github.com/UTEP-Dynamic-Materials-Lab/SHPB_Toolkit/tree/main/ontology#hasAffiliation
:hasAffiliation rdf:type owl:DatatypeProperty ;
                rdfs:domain :Laboratory ,
                            :User ;
                rdfs:range xsd:string ;
                rdfs:comment "Specifies the institution or organization the laboratory is affiliated with." .


###  https://github.com/UTEP-Dynamic-Materials-Lab/SHPB_Toolkit/tree/main/ontology#hasChemicalComposition
:hasChemicalComposition rdf:type owl:DatatypeProperty ;
                        rdfs:domain :Material ;
                        rdfs:range xsd:string ;
                        rdfs:comment "Specifies the chemical composition of the specimen." .


###  https://github.com/UTEP-Dynamic-Materials-Lab/SHPB_Toolkit/tree/main/ontology#hasDescription
:hasDescription rdf:type owl:DatatypeProperty ;
                rdfs:range xsd:string .


###  https://github.com/UTEP-Dynamic-Materials-Lab/SHPB_Toolkit/tree/main/ontology#hasEncodedData
:hasEncodedData rdf:type owl:DatatypeProperty ;
                rdfs:subPropertyOf owl:topDataProperty ;
                rdfs:domain :ExtractedSignal ,
                            :SensorSignal ,
                            :SeriesData ;
                rdfs:range xsd:base64Binary .


###  https://github.com/UTEP-Dynamic-Materials-Lab/SHPB_Toolkit/tree/main/ontology#hasEncoding
:hasEncoding rdf:type owl:DatatypeProperty ;
             rdfs:range xsd:string ;
             rdfs:comment "Specifies the encoding used for storing the data, such as 'Base64'." .


###  https://github.com/UTEP-Dynamic-Materials-Lab/SHPB_Toolkit/tree/main/ontology#hasLegendName
:hasLegendName rdf:type owl:DatatypeProperty ;
               rdfs:range xsd:string ;
               rdfs:comment "Gives a human-readable name for the series or scalar value." .


###  https://github.com/UTEP-Dynamic-Materials-Lab/SHPB_Toolkit/tree/main/ontology#hasLocation
:hasLocation rdf:type owl:DatatypeProperty ;
             rdfs:domain :Laboratory ;
             rdfs:range xsd:string ;
             rdfs:comment "Specifies the location of the laboratory, e.g., Building A, Room 12." .


###  https://github.com/UTEP-Dynamic-Materials-Lab/SHPB_Toolkit/tree/main/ontology#hasName
:hasName rdf:type owl:DatatypeProperty .


###  https://github.com/UTEP-Dynamic-Materials-Lab/SHPB_Toolkit/tree/main/ontology#hasSize
:hasSize rdf:type owl:DatatypeProperty ;
         rdfs:range xsd:integer ;
         rdfs:comment "Indicates the size of the dataset, such as the number of points in a series." .


###  https://github.com/UTEP-Dynamic-Materials-Lab/SHPB_Toolkit/tree/main/ontology#hasSupervisor
:hasSupervisor rdf:type owl:DatatypeProperty ;
               rdfs:domain :Laboratory ;
               rdfs:range xsd:string ;
               rdfs:comment "Specifies the name of the test supervisor." .


###  https://github.com/UTEP-Dynamic-Materials-Lab/SHPB_Toolkit/tree/main/ontology#hasSymbol
:hasSymbol rdf:type owl:DatatypeProperty ;
           rdfs:range xsd:string ;
           rdfs:comment "Provides the LaTeX symbol for use in plotting or labeling." .


###  https://github.com/UTEP-Dynamic-Materials-Lab/SHPB_Toolkit/tree/main/ontology#hasTestDate
:hasTestDate rdf:type owl:DatatypeProperty ;
             rdfs:domain :Metadata ;
             rdfs:range xsd:date ;
             rdfs:comment "Specifies the date the test was performed." .


###  https://github.com/UTEP-Dynamic-Materials-Lab/SHPB_Toolkit/tree/main/ontology#hasTestName
:hasTestName rdf:type owl:DatatypeProperty ;
             rdfs:domain :Metadata ;
             rdfs:range xsd:string ;
             rdfs:comment "Specifies the name of the test." .


###  https://github.com/UTEP-Dynamic-Materials-Lab/SHPB_Toolkit/tree/main/ontology#hasValue
:hasValue rdf:type owl:DatatypeProperty ;
          rdfs:range xsd:float ;
          rdfs:comment "Stores the numerical value of a scalar property, such as UTS." .


#################################################################
#    Classes
#################################################################

###  https://github.com/UTEP-Dynamic-Materials-Lab/SHPB_Toolkit/tree/main/ontology#AluminiumAlloy
:AluminiumAlloy rdf:type owl:Class ;
                rdfs:subClassOf :Material ;
                rdfs:comment "The general class thats hosts Aluminium engineering alloys." .


###  https://github.com/UTEP-Dynamic-Materials-Lab/SHPB_Toolkit/tree/main/ontology#AreaUnit
:AreaUnit rdf:type owl:Class ;
          rdfs:subClassOf :Unit ;
          rdfs:comment "Represents units of area" .


###  https://github.com/UTEP-Dynamic-Materials-Lab/SHPB_Toolkit/tree/main/ontology#Bar
:Bar rdf:type owl:Class ;
     rdfs:subClassOf :TestingConditions ;
     rdfs:comment "Describes the bar utilized in SHPB testing. Includes instances for Incident, Striker and Transmitted Bars" .


###  https://github.com/UTEP-Dynamic-Materials-Lab/SHPB_Toolkit/tree/main/ontology#CompositeMaterial
:CompositeMaterial rdf:type owl:Class ;
                   rdfs:subClassOf :Material .


###  https://github.com/UTEP-Dynamic-Materials-Lab/SHPB_Toolkit/tree/main/ontology#CopperAlloy
:CopperAlloy rdf:type owl:Class ;
             rdfs:subClassOf :Material ;
             rdfs:comment "The general class thats hosts Copper engineering alloys" .


###  https://github.com/UTEP-Dynamic-Materials-Lab/SHPB_Toolkit/tree/main/ontology#DensityUnit
:DensityUnit rdf:type owl:Class ;
             rdfs:subClassOf :Unit ;
             rdfs:comment "Represents units of density" .


###  https://github.com/UTEP-Dynamic-Materials-Lab/SHPB_Toolkit/tree/main/ontology#Dimension
:Dimension rdf:type owl:Class ;
           rdfs:comment "Represents numerical values that defines the geometric characteristics or measurable extents of an object or system. Typically described in terms of length, width, height, and time." .


###  https://github.com/UTEP-Dynamic-Materials-Lab/SHPB_Toolkit/tree/main/ontology#ElectricPotentialUnit
:ElectricPotentialUnit rdf:type owl:Class ;
                       rdfs:subClassOf :Unit ;
                       rdfs:comment "Represents units of electric potential" .


###  https://github.com/UTEP-Dynamic-Materials-Lab/SHPB_Toolkit/tree/main/ontology#ElectricalResistanceUnit
:ElectricalResistanceUnit rdf:type owl:Class ;
                          rdfs:subClassOf :Unit ;
                          rdfs:comment "Represents units of electrical resistance" .


###  https://github.com/UTEP-Dynamic-Materials-Lab/SHPB_Toolkit/tree/main/ontology#EnergyUnit
:EnergyUnit rdf:type owl:Class ;
            rdfs:subClassOf :Unit ;
            rdfs:comment "Represents units of energy" .


###  https://github.com/UTEP-Dynamic-Materials-Lab/SHPB_Toolkit/tree/main/ontology#Experiment
:Experiment rdf:type owl:Class ;
            rdfs:comment "A systematic method to determine the mechanical response of materials. Each instance of the class represents a different experimental method." .


###  https://github.com/UTEP-Dynamic-Materials-Lab/SHPB_Toolkit/tree/main/ontology#ExtractedSignal
:ExtractedSignal rdf:type owl:Class ;
                 rdfs:subClassOf :SecondaryData ;
                 rdfs:comment "Represents the extracted signals that relates to the pulse duration during SHPB analysis." .


###  https://github.com/UTEP-Dynamic-Materials-Lab/SHPB_Toolkit/tree/main/ontology#FEAMetadata
:FEAMetadata rdf:type owl:Class ;
             rdfs:comment "Description of the attributes and processes used to describe the objects / forces in a finite element (FE) analysis. Including structured reference to strenght models and element definitions" .


###  https://github.com/UTEP-Dynamic-Materials-Lab/SHPB_Toolkit/tree/main/ontology#FiniteElement
:FiniteElement rdf:type owl:Class ;
               rdfs:subClassOf :FEAMetadata ;
               rdfs:comment "Describes the type of element used in FE analysis. Includes definitions for 2D and 3D elements with respective documentation." .


###  https://github.com/UTEP-Dynamic-Materials-Lab/SHPB_Toolkit/tree/main/ontology#ForceUnit
:ForceUnit rdf:type owl:Class ;
           rdfs:subClassOf :Unit .


###  https://github.com/UTEP-Dynamic-Materials-Lab/SHPB_Toolkit/tree/main/ontology#FrequencyUnit
:FrequencyUnit rdf:type owl:Class ;
               rdfs:subClassOf :Unit ;
               rdfs:comment "Represents time dependent units" .


###  https://github.com/UTEP-Dynamic-Materials-Lab/SHPB_Toolkit/tree/main/ontology#Laboratory
:Laboratory rdf:type owl:Class ;
            rdfs:subClassOf :Metadata ;
            rdfs:comment "Describes the laboratories where experiments takes place." .


###  https://github.com/UTEP-Dynamic-Materials-Lab/SHPB_Toolkit/tree/main/ontology#LengthUnit
:LengthUnit rdf:type owl:Class ;
            rdfs:subClassOf :Unit ;
            rdfs:comment "Represents units of length" .


###  https://github.com/UTEP-Dynamic-Materials-Lab/SHPB_Toolkit/tree/main/ontology#Material
:Material rdf:type owl:Class ;
          rdfs:comment "Represents the engineering materials used for testing. Includes a sub-level alloy categories followed by individual instances of those alloys." .


###  https://github.com/UTEP-Dynamic-Materials-Lab/SHPB_Toolkit/tree/main/ontology#MechanicalProperty
:MechanicalProperty rdf:type owl:Class ;
                    rdfs:comment "Represents a mechanical property that characterizes the material behavior, such as elastic modulus or density. Properties are either defined or calculated during experiments. Also doubles as the paramaters for strength models." .


###  https://github.com/UTEP-Dynamic-Materials-Lab/SHPB_Toolkit/tree/main/ontology#Metadata
:Metadata rdf:type owl:Class ;
          rdfs:comment "Captures general values of testing conditions, test specimen, user and laboratory used during an experiment. Used as the main context to perform queries." .


###  https://github.com/UTEP-Dynamic-Materials-Lab/SHPB_Toolkit/tree/main/ontology#MomentumTrap
:MomentumTrap rdf:type owl:Class ;
              rdfs:subClassOf :TestingConditions ;
              rdfs:comment "Describes the condition of the Momentum Trap in a SHPB experiment. Guides post-process analysis." .


###  https://github.com/UTEP-Dynamic-Materials-Lab/SHPB_Toolkit/tree/main/ontology#PressureUnit
:PressureUnit rdf:type owl:Class ;
              rdfs:subClassOf :Unit ;
              rdfs:comment "Represents units of pressure" .


###  https://github.com/UTEP-Dynamic-Materials-Lab/SHPB_Toolkit/tree/main/ontology#PrimaryData
:PrimaryData rdf:type owl:Class ;
             rdfs:comment "Represents raw data directly collected during the experiment from sensors, including strain gauges, time and temperature." .


###  https://github.com/UTEP-Dynamic-Materials-Lab/SHPB_Toolkit/tree/main/ontology#PulseProperties
:PulseProperties rdf:type owl:Class ;
                 rdfs:subClassOf :SecondaryData ;
                 rdfs:comment "Represents determined pulse properties as a result of testing conditions in a SHPB experiment" .


###  https://github.com/UTEP-Dynamic-Materials-Lab/SHPB_Toolkit/tree/main/ontology#SecondaryData
:SecondaryData rdf:type owl:Class ;
               rdfs:comment "Represents processed data and determined mechanical properties, including series and single-value properties." .


###  https://github.com/UTEP-Dynamic-Materials-Lab/SHPB_Toolkit/tree/main/ontology#SensorSignal
:SensorSignal rdf:type owl:Class ;
              rdfs:subClassOf :PrimaryData ;
              rdfs:comment "Represents a generic signal from a sensor." .


###  https://github.com/UTEP-Dynamic-Materials-Lab/SHPB_Toolkit/tree/main/ontology#SeriesData
:SeriesData rdf:type owl:Class ;
            rdfs:subClassOf :SecondaryData ;
            rdfs:comment "Represents a generic data series, such as stress or strain." .


###  https://github.com/UTEP-Dynamic-Materials-Lab/SHPB_Toolkit/tree/main/ontology#Shape
:Shape rdf:type owl:Class ;
       rdfs:subClassOf :Specimen ;
       rdfs:comment "Describes the shape of the tested specimen." .


###  https://github.com/UTEP-Dynamic-Materials-Lab/SHPB_Toolkit/tree/main/ontology#Specimen
:Specimen rdf:type owl:Class ;
          rdfs:subClassOf :Metadata ;
          rdfs:comment "Describes the specimen tested, including its material and geometry." .


###  https://github.com/UTEP-Dynamic-Materials-Lab/SHPB_Toolkit/tree/main/ontology#SpecimenProcessing
:SpecimenProcessing rdf:type owl:Class ;
                    rdfs:subClassOf :Specimen ;
                    rdfs:comment "Represents the engineering processing methods utilized on materials. In general, describe the manufacturing and heat treatment state of materials used in the experiments." .


###  https://github.com/UTEP-Dynamic-Materials-Lab/SHPB_Toolkit/tree/main/ontology#SteelAlloy
:SteelAlloy rdf:type owl:Class ;
            rdfs:subClassOf :Material ;
            rdfs:comment "The general class thats hosts Steel engineering alloys." .


###  https://github.com/UTEP-Dynamic-Materials-Lab/SHPB_Toolkit/tree/main/ontology#StrainGauge
:StrainGauge rdf:type owl:Class ;
             rdfs:comment "Refers to the strain gauge used in experiments" .


###  https://github.com/UTEP-Dynamic-Materials-Lab/SHPB_Toolkit/tree/main/ontology#StrainGaugeProperties
:StrainGaugeProperties rdf:type owl:Class ;
                       rdfs:subClassOf :StrainGauge ;
                       rdfs:comment "Captures all properties related to strain gauge calibration." .


###  https://github.com/UTEP-Dynamic-Materials-Lab/SHPB_Toolkit/tree/main/ontology#StrengthModel
:StrengthModel rdf:type owl:Class ;
               rdfs:subClassOf :FEAMetadata ;
               rdfs:comment "Represents the strength model used in FE analysis. Includes the definition of the required parameters." .


###  https://github.com/UTEP-Dynamic-Materials-Lab/SHPB_Toolkit/tree/main/ontology#Structure
:Structure rdf:type owl:Class ;
           rdfs:subClassOf :Specimen ;
           rdfs:comment "Describes the macro-scale ( > 10^-1) or meso-scale (10^-5 - 10^-1) physical structure of the specimen. Intended to evaluate the material's reponse under different pyshical representations" .


###  https://github.com/UTEP-Dynamic-Materials-Lab/SHPB_Toolkit/tree/main/ontology#TemperatureUnit
:TemperatureUnit rdf:type owl:Class ;
                 rdfs:subClassOf :Unit ;
                 rdfs:comment "Represents units of temperature" .


###  https://github.com/UTEP-Dynamic-Materials-Lab/SHPB_Toolkit/tree/main/ontology#TestMode
:TestMode rdf:type owl:Class ;
          rdfs:subClassOf :TestingConditions ;
          rdfs:comment "Describes the mode in which a experiment takes place, including FEA and Lab analysis modes." .


###  https://github.com/UTEP-Dynamic-Materials-Lab/SHPB_Toolkit/tree/main/ontology#TestTemperature
:TestTemperature rdf:type owl:Class ;
                 rdfs:subClassOf :TestingConditions ;
                 rdfs:comment "Describes the test temperature used in experiments" .


###  https://github.com/UTEP-Dynamic-Materials-Lab/SHPB_Toolkit/tree/main/ontology#TestType
:TestType rdf:type owl:Class ;
          rdfs:subClassOf :TestingConditions ;
          rdfs:comment "Represents the type of test conducted, such as pulse, calibration or specimen testing." .


###  https://github.com/UTEP-Dynamic-Materials-Lab/SHPB_Toolkit/tree/main/ontology#TestingConditions
:TestingConditions rdf:type owl:Class ;
                   rdfs:subClassOf :Metadata ;
                   rdfs:comment "Describes the test components used to make an experiment happen. Such as descriptors for the test equipments, FEA / Lab analysis, test temperature and calibration procedures" .


###  https://github.com/UTEP-Dynamic-Materials-Lab/SHPB_Toolkit/tree/main/ontology#TimeUnit
:TimeUnit rdf:type owl:Class ;
          rdfs:subClassOf :Unit ;
          rdfs:comment "Represents units of time" .


###  https://github.com/UTEP-Dynamic-Materials-Lab/SHPB_Toolkit/tree/main/ontology#Unit
:Unit rdf:type owl:Class ;
      rdfs:comment "Represents the general class of a physical unit of measurement." .


###  https://github.com/UTEP-Dynamic-Materials-Lab/SHPB_Toolkit/tree/main/ontology#UnitlessUnit
:UnitlessUnit rdf:type owl:Class ;
              rdfs:subClassOf :Unit ;
              rdfs:comment "Represents rational (unitless) units" .


###  https://github.com/UTEP-Dynamic-Materials-Lab/SHPB_Toolkit/tree/main/ontology#User
:User rdf:type owl:Class ;
      rdfs:subClassOf :Metadata ;
      rdfs:comment "Represents a user involved in the experiment. Also refers to the person which validates the entry of the data." .


###  https://github.com/UTEP-Dynamic-Materials-Lab/SHPB_Toolkit/tree/main/ontology#VelocityUnit
:VelocityUnit rdf:type owl:Class ;
              rdfs:subClassOf :Unit ;
              rdfs:comment "Represents units of velocity or speed" .


###  https://github.com/UTEP-Dynamic-Materials-Lab/SHPB_Toolkit/tree/main/ontology#VolumeUnit
:VolumeUnit rdf:type owl:Class ;
            rdfs:subClassOf :Unit ;
            rdfs:comment "Represents units of volume" .


###  https://github.com/UTEP-Dynamic-Materials-Lab/SHPB_Toolkit/tree/main/ontology#2DElement
<https://github.com/UTEP-Dynamic-Materials-Lab/SHPB_Toolkit/tree/main/ontology#2DElement> rdf:type owl:Class ;
                                                                                          rdfs:subClassOf :FiniteElement ;
                                                                                          rdfs:comment "Represents 2D Finite Element types in comercially availbale softwares" .


###  https://github.com/UTEP-Dynamic-Materials-Lab/SHPB_Toolkit/tree/main/ontology#3DElement
<https://github.com/UTEP-Dynamic-Materials-Lab/SHPB_Toolkit/tree/main/ontology#3DElement> rdf:type owl:Class ;
                                                                                          rdfs:subClassOf :FiniteElement ;
                                                                                          rdfs:comment "Represents 3D Finite Element types in comercially availbale softwares" .


#################################################################
#    Individuals
#################################################################

###  https://github.com/UTEP-Dynamic-Materials-Lab/SHPB_Toolkit/tree/main/ontology#A356
:A356 rdf:type owl:NamedIndividual ,
               :AluminiumAlloy ;
      :hasAbbreviation "A356" ;
      :hasLegendName "Al 356 Alloy" ;
      :hasName "Aluminium A356 Alloy" .


###  https://github.com/UTEP-Dynamic-Materials-Lab/SHPB_Toolkit/tree/main/ontology#AL6061T6
:AL6061T6 rdf:type owl:NamedIndividual ,
                   :AluminiumAlloy ;
          :hasAbbreviation "AL6061T6" ;
          :hasLegendName "AL6061-T6 Alloy" ;
          :hasName "Aluminum 6061-T6 Alloy" .


###  https://github.com/UTEP-Dynamic-Materials-Lab/SHPB_Toolkit/tree/main/ontology#AL7075T6
:AL7075T6 rdf:type owl:NamedIndividual ,
                   :AluminiumAlloy ;
          :hasAbbreviation "AL7075T6" ;
          :hasLegendName "AL7075-T6 Alloy" ;
          :hasName "Aluminum 7075-T6 Alloy" .


###  https://github.com/UTEP-Dynamic-Materials-Lab/SHPB_Toolkit/tree/main/ontology#AbsorbedEnergy
:AbsorbedEnergy rdf:type owl:NamedIndividual ,
                         :SeriesData ;
                rdfs:comment "Represents absorbed energy series data." .


###  https://github.com/UTEP-Dynamic-Materials-Lab/SHPB_Toolkit/tree/main/ontology#AnnealingHT
:AnnealingHT rdf:type owl:NamedIndividual ;
             :hasAbbreviation "Annealed Alloy" ;
             :hasName "Annealed Alloy" .


###  https://github.com/UTEP-Dynamic-Materials-Lab/SHPB_Toolkit/tree/main/ontology#BelytschkoTsay
:BelytschkoTsay rdf:type owl:NamedIndividual ,
                         <https://github.com/UTEP-Dynamic-Materials-Lab/SHPB_Toolkit/tree/main/ontology#2DElement> ;
                :hasDimension :ElementSize ;
                :hasAbbreviation "Belytschko-Tsay Element" ;
                rdfs:comment "Represents the Belytschko Tsay shell element in LS-Dyna" ;
                :hasName "Belytschko Tsay 2D Shell Element" .


###  https://github.com/UTEP-Dynamic-Materials-Lab/SHPB_Toolkit/tree/main/ontology#Brass414
:Brass414 rdf:type owl:NamedIndividual ,
                   :CopperAlloy ;
          :hasAbbreviation "CU414HO2" ;
          :hasLegendName "Brass 414 H02 Alloy" ;
          :hasName "Brass 414 H02 Alloy" .


###  https://github.com/UTEP-Dynamic-Materials-Lab/SHPB_Toolkit/tree/main/ontology#BrianSchuster
:BrianSchuster rdf:type owl:NamedIndividual ,
                        :User ;
               :hasAbbreviation "BES" ;
               :hasAffiliation "The University of Texas at El Paso" ;
               :hasLocation "PHYS Building, Room 412" ;
               :hasName "Brian E. Schuster" .


###  https://github.com/UTEP-Dynamic-Materials-Lab/SHPB_Toolkit/tree/main/ontology#CU101
:CU101 rdf:type owl:NamedIndividual ,
                :CopperAlloy ;
       :hasAbbreviation "CU101" ;
       :hasLegendName "Cu101 Alloy" ;
       :hasName "Copper 101 Alloy" .


###  https://github.com/UTEP-Dynamic-Materials-Lab/SHPB_Toolkit/tree/main/ontology#CalibrationResistance
:CalibrationResistance rdf:type owl:NamedIndividual ,
                                :StrainGaugeProperties ;
                       :hasUnits :MilliOhms ,
                                 :Ohms ;
                       rdfs:comment "Represents the calibration resistance of the strain gauge in ohms." ;
                       :hasName "Strain Gauge Calibration Resistance" .


###  https://github.com/UTEP-Dynamic-Materials-Lab/SHPB_Toolkit/tree/main/ontology#CalibrationVoltage
:CalibrationVoltage rdf:type owl:NamedIndividual ,
                             :StrainGaugeProperties ;
                    :hasUnits :MilliVolts ,
                              :Volts ;
                    rdfs:comment "Represents the calibration voltage of the strain gauge in volts." ;
                    :hasName "Strain Gauge Calibration Voltage" .


###  https://github.com/UTEP-Dynamic-Materials-Lab/SHPB_Toolkit/tree/main/ontology#CastingProcess
:CastingProcess rdf:type owl:NamedIndividual ,
                         :SpecimenProcessing ;
                :hasAbbreviation "Casted Specimen" ;
                rdfs:comment "Refers to a specimen that was casted. Commonly used in SHPB testing." ;
                :hasName "Casted Material" .


###  https://github.com/UTEP-Dynamic-Materials-Lab/SHPB_Toolkit/tree/main/ontology#Cubic
:Cubic rdf:type owl:NamedIndividual ,
                :Shape ;
       :hasAbbreviation "CUB" ;
       rdfs:comment "Cubic shaped specimens, not commonly used in SHPB testing." ;
       :hasName "Cubic Shape" .


###  https://github.com/UTEP-Dynamic-Materials-Lab/SHPB_Toolkit/tree/main/ontology#CubicCentimeter
:CubicCentimeter rdf:type owl:NamedIndividual ,
                          :VolumeUnit ;
                 :hasAbbreviation "$\\text{cm}^3$" ;
                 :hasSymbol "$\\text{cm}^3$" ;
                 rdfs:comment "Cubic centimeter, a unit of volume in the SI system." .


###  https://github.com/UTEP-Dynamic-Materials-Lab/SHPB_Toolkit/tree/main/ontology#CubicFoot
:CubicFoot rdf:type owl:NamedIndividual ,
                    :VolumeUnit ;
           :hasAbbreviation "\\text{ft}^3" ;
           :hasSymbol "$\\text{ft}^3$" ;
           rdfs:comment "Cubic foot, a unit of volume in the English system." .


###  https://github.com/UTEP-Dynamic-Materials-Lab/SHPB_Toolkit/tree/main/ontology#CubicInch
:CubicInch rdf:type owl:NamedIndividual ,
                    :VolumeUnit ;
           :hasAbbreviation "in^3" ;
           :hasSymbol "$\\text{in}^3$" ;
           rdfs:comment "Cubic inch, a unit of volume in the English system." .


###  https://github.com/UTEP-Dynamic-Materials-Lab/SHPB_Toolkit/tree/main/ontology#CubicMeter
:CubicMeter rdf:type owl:NamedIndividual ,
                     :VolumeUnit ;
            :hasAbbreviation "$m^3$" ;
            :hasSymbol "$\\text{m}^3$" ;
            rdfs:comment "Cubic meter, a unit of volume in the SI system." .


###  https://github.com/UTEP-Dynamic-Materials-Lab/SHPB_Toolkit/tree/main/ontology#CubicMillimeter
:CubicMillimeter rdf:type owl:NamedIndividual ,
                          :VolumeUnit ;
                 :hasAbbreviation "mm^3" ;
                 :hasSymbol "$\\text{mm}^3$" ;
                 rdfs:comment "Cubic millimeter, a unit of volume in the SI system." .


###  https://github.com/UTEP-Dynamic-Materials-Lab/SHPB_Toolkit/tree/main/ontology#Cylindrical
:Cylindrical rdf:type owl:NamedIndividual ,
                      :Shape ;
             :hasAbbreviation "CYL" ;
             rdfs:comment "Cylindrical shaped test specimens, commonly used in SHPB testing." ;
             :hasName "Cylindrical Shape" .


###  https://github.com/UTEP-Dynamic-Materials-Lab/SHPB_Toolkit/tree/main/ontology#DataAcquisitionRate
:DataAcquisitionRate rdf:type owl:NamedIndividual ,
                              :StrainGaugeProperties ;
                     :hasUnits :GigaHertz ,
                               :Hertz ,
                               :KiloHertz ,
                               :MegaHertz ;
                     :hasLegendName "DAQ" ;
                     rdfs:comment "Represents the data acquisition rate for the sensors" ;
                     :hasName "Data Acquisition Rate" .


###  https://github.com/UTEP-Dynamic-Materials-Lab/SHPB_Toolkit/tree/main/ontology#DavidSantacruz
:DavidSantacruz rdf:type owl:NamedIndividual ,
                         :User ;
                :hasAbbreviation "DKS" ;
                :hasAffiliation "The University of Texas at El Paso" ;
                :hasLocation "PHYS Building, Room 412" ;
                :hasSupervisor "Brian E. Schuster" ;
                :hasName "David K. Santacruz" .


###  https://github.com/UTEP-Dynamic-Materials-Lab/SHPB_Toolkit/tree/main/ontology#DeformedCrossSectionalArea
:DeformedCrossSectionalArea rdf:type owl:NamedIndividual ,
                                     :Dimension ;
                            :hasUnits :SquareInches ,
                                      :SquareMeters ,
                                      :SquareMilimeters ;
                            :hasAbbreviation "Deformed Cross Section" ;
                            :hasName "Deformed Cross Sectional Area" .


###  https://github.com/UTEP-Dynamic-Materials-Lab/SHPB_Toolkit/tree/main/ontology#DeformedDiameter
:DeformedDiameter rdf:type owl:NamedIndividual ,
                           :Dimension ;
                  :hasUnits :Foot ,
                            :Inch ,
                            :Meter ,
                            :Micrometer ,
                            :Millimeter ;
                  :hasAbbreviation "Deformed Diameter" ;
                  :hasName "Deformed Diameter" .


###  https://github.com/UTEP-Dynamic-Materials-Lab/SHPB_Toolkit/tree/main/ontology#DeformedLength
:DeformedLength rdf:type owl:NamedIndividual ,
                         :Dimension ;
                :hasUnits :Foot ,
                          :Inch ,
                          :Meter ,
                          :Micrometer ,
                          :Millimeter ;
                :hasAbbreviation "Deformed Lentgth" ;
                :hasName "Deformed Length" .


###  https://github.com/UTEP-Dynamic-Materials-Lab/SHPB_Toolkit/tree/main/ontology#DegreesCelsius
:DegreesCelsius rdf:type owl:NamedIndividual ,
                         :TemperatureUnit ;
                :hasAbbreviation "C" ;
                :hasSymbol "$\\dot{C}$" .


###  https://github.com/UTEP-Dynamic-Materials-Lab/SHPB_Toolkit/tree/main/ontology#DegressFahrenheit
:DegressFahrenheit rdf:type owl:NamedIndividual ,
                            :TemperatureUnit ;
                   :hasAbbreviation "F" ;
                   :hasSymbol "$\\dot{F}$" .


###  https://github.com/UTEP-Dynamic-Materials-Lab/SHPB_Toolkit/tree/main/ontology#Density
:Density rdf:type owl:NamedIndividual ,
                  :MechanicalProperty ;
         :hasUnits :GramPerCubicMillimeter ,
                   :KilogramPerCubicMeter ,
                   :KilogramPerCubicMillimeter ;
         :hasSymbol "$\\rho$" ;
         rdfs:comment "The mass per unit volume of the material." ,
                      "This dimension was moved to the Mechanical Property because most strength models use density as a parameter. And hasParameter points to a Mechcanical Property" ;
         :hasName "Density" .


###  https://github.com/UTEP-Dynamic-Materials-Lab/SHPB_Toolkit/tree/main/ontology#DynaMatLab
:DynaMatLab rdf:type owl:NamedIndividual ,
                     :Laboratory ;
            :hasAbbreviation "Dynamic Materials Laboratory" ;
            :hasAffiliation "University of Texas at El Paso" ;
            :hasLocation "PHYS Building, Room 412" ;
            :hasSupervisor "Dr Brian E Schuster" ;
            :hasName "Dynamic Material's Laboratory" .


###  https://github.com/UTEP-Dynamic-Materials-Lab/SHPB_Toolkit/tree/main/ontology#ElasticModulus
:ElasticModulus rdf:type owl:NamedIndividual ,
                         :MechanicalProperty ;
                :hasUnits :Gigapascal ,
                          :Megapascal ,
                          :Pascal ,
                          :Psi ;
                :hasSymbol "$E$" ;
                rdfs:comment "Represents the stiffness of the material in the elastic range. Measured as the linear portion of a stress-strain graph" ;
                :hasName "Elastic Modulus" .


###  https://github.com/UTEP-Dynamic-Materials-Lab/SHPB_Toolkit/tree/main/ontology#ElasticStrengthModel
:ElasticStrengthModel rdf:type owl:NamedIndividual ,
                               :StrengthModel ;
                      :hasParameter :Density ,
                                    :ElasticModulus ,
                                    :PoissonsRatio ;
                      :hasAbbreviation "Elastic Model" ;
                      rdfs:comment "Represents the Elastic Model, MAT 001, from LS Dyna" ;
                      :hasName "Elastic Strength Model" .


###  https://github.com/UTEP-Dynamic-Materials-Lab/SHPB_Toolkit/tree/main/ontology#ElementSize
:ElementSize rdf:type owl:NamedIndividual ,
                      :Dimension ;
             :hasUnits :Foot ,
                       :Inch ,
                       :Meter ,
                       :Micrometer ,
                       :Millimeter ,
                       :SquareInches ,
                       :SquareMeters ,
                       :SquareMilimeters ;
             :hasAbbreviation "FE Size" ;
             :hasName "Finite Element Size" .


###  https://github.com/UTEP-Dynamic-Materials-Lab/SHPB_Toolkit/tree/main/ontology#EmilioLoera
:EmilioLoera rdf:type owl:NamedIndividual ,
                      :User ;
             :hasAbbreviation "ESL" ;
             :hasAffiliation "University of Texas at El Paso" ;
             :hasLocation "PHYS Buiding, Room 412" ;
             :hasSupervisor "Brian E. Schuster" ;
             :hasName "Emilio S. Loera" .


###  https://github.com/UTEP-Dynamic-Materials-Lab/SHPB_Toolkit/tree/main/ontology#EngineeringStrain
:EngineeringStrain rdf:type owl:NamedIndividual ,
                            :SeriesData ;
                   :hasSymbol "$\\varepsilon$" ;
                   rdfs:comment "Represents engineering strain series data." ;
                   :hasName "Engineering Strain" .


###  https://github.com/UTEP-Dynamic-Materials-Lab/SHPB_Toolkit/tree/main/ontology#EngineeringStrainRate
:EngineeringStrainRate rdf:type owl:NamedIndividual ,
                                :SeriesData ;
                       :hasSymbol "$\\dot{\\varepsilon}$" ;
                       rdfs:comment "Represents engineering strain rate series data." ;
                       :hasName "Engineering Strain Rate" .


###  https://github.com/UTEP-Dynamic-Materials-Lab/SHPB_Toolkit/tree/main/ontology#EngineeringStress
:EngineeringStress rdf:type owl:NamedIndividual ,
                            :SeriesData ;
                   :hasSymbol "$\\sigma$" ;
                   rdfs:comment "Represents engineering stress series data." ;
                   :hasName "Engineering Stress" .


###  https://github.com/UTEP-Dynamic-Materials-Lab/SHPB_Toolkit/tree/main/ontology#ErwinCazares
:ErwinCazares rdf:type owl:NamedIndividual ,
                       :User ;
              :hasAbbreviation "ECG" ;
              :hasAffiliation "University of Texas at El Paso" ;
              :hasLocation "PHYS Building, Room 412" ;
              :hasSupervisor "Brian E. Schuster" ;
              :hasName "Erwin Cazares" .


###  https://github.com/UTEP-Dynamic-Materials-Lab/SHPB_Toolkit/tree/main/ontology#FEAMode
:FEAMode rdf:type owl:NamedIndividual ,
                  :TestMode ;
         :hasAbbreviation "FEA" ;
         rdfs:comment "Indicates that the experiment was done using simulated testing conditions." ;
         :hasName "FEA Testing Conditions" .


###  https://github.com/UTEP-Dynamic-Materials-Lab/SHPB_Toolkit/tree/main/ontology#Foot
:Foot rdf:type owl:NamedIndividual ,
               :LengthUnit ;
      :hasAbbreviation "ft" ;
      :hasSymbol "$ft$" ;
      rdfs:comment "Foot, a unit of length in the English system." .


###  https://github.com/UTEP-Dynamic-Materials-Lab/SHPB_Toolkit/tree/main/ontology#FootPerSecond
:FootPerSecond rdf:type owl:NamedIndividual ,
                        :VelocityUnit ;
               :hasAbbreviation "ft/s" ;
               :hasSymbol "$\\frac{ft}{s}$" ;
               rdfs:comment "Foot per second, a unit of velocity in the English system." .


###  https://github.com/UTEP-Dynamic-Materials-Lab/SHPB_Toolkit/tree/main/ontology#GaugeFactor
:GaugeFactor rdf:type owl:NamedIndividual ,
                      :StrainGaugeProperties ;
             :hasUnits :Unitless ;
             rdfs:comment "Represents the gauge factor of the strain gauge." ;
             :hasName "Strain Gauge Factor" .


###  https://github.com/UTEP-Dynamic-Materials-Lab/SHPB_Toolkit/tree/main/ontology#GigaHertz
:GigaHertz rdf:type owl:NamedIndividual ,
                    :FrequencyUnit ;
           :hasAbbreviation "GHz" ;
           :hasSymbol "$GHz$" .


###  https://github.com/UTEP-Dynamic-Materials-Lab/SHPB_Toolkit/tree/main/ontology#Gigapascal
:Gigapascal rdf:type owl:NamedIndividual ,
                     :PressureUnit ;
            :hasAbbreviation "GPa" ;
            :hasSymbol "$\\text{GPa}$" ;
            rdfs:comment "Gigapascal, a unit of pressure in the SI system." .


###  https://github.com/UTEP-Dynamic-Materials-Lab/SHPB_Toolkit/tree/main/ontology#GramPerCubicMillimeter
:GramPerCubicMillimeter rdf:type owl:NamedIndividual ,
                                 :DensityUnit ;
                        :hasAbbreviation "g/mm^3" ;
                        :hasSymbol "$\\frac{g}{mm^3}$" ;
                        rdfs:comment "Gram per cubic millimeter, a unit of density." .


###  https://github.com/UTEP-Dynamic-Materials-Lab/SHPB_Toolkit/tree/main/ontology#GyroidLattice
:GyroidLattice rdf:type owl:NamedIndividual ,
                        :Structure ;
               :hasAbbreviation "GYR" ;
               rdfs:comment "A gyroid structure is a 3D structure of triply periodic minimal surface (TPMS), which means it has a zero mean curvature and locally minimizes area, also characterized to only present one continous surface." ,
                            "Defined by the formula: > f(x, y, z) = sin(x)cos(y) + sin(y)cos(z) + sin(z)cos(x)" ;
               :hasName "Gyroid Lattice" .


###  https://github.com/UTEP-Dynamic-Materials-Lab/SHPB_Toolkit/tree/main/ontology#HardeningExponent
:HardeningExponent rdf:type owl:NamedIndividual ,
                            :MechanicalProperty ;
                   :hasUnits :Unitless ;
                   :hasSymbol "$n$" ;
                   rdfs:comment "Hardening exponent of the material. Characterizes the strain hardening of a material during the forming process. Defined by the gradient of the flow curve in a double-logarithmic form." ,
                                "Represents the parameter \"n\" in LS-Dyna JC Simplified model" ;
                   :hasName "Hardening Exponent" .


###  https://github.com/UTEP-Dynamic-Materials-Lab/SHPB_Toolkit/tree/main/ontology#HardeningModulus
:HardeningModulus rdf:type owl:NamedIndividual ,
                           :MechanicalProperty ;
                  :hasUnits :Gigapascal ,
                            :Megapascal ,
                            :Pascal ,
                            :Psi ;
                  :hasSymbol "$B$" ;
                  rdfs:comment "Hardening modulus of the material. Determined as the slope of the stress vs plastic strain curve. Represents the resistance of a material to continue plastic deformation. Commonly used in constitutive elastoplastic equations." ,
                               "Represents the parameter \"b\" in LS Dyna JC Simplified Model" ;
                  :hasName "Hardening Modulus" .


###  https://github.com/UTEP-Dynamic-Materials-Lab/SHPB_Toolkit/tree/main/ontology#Hertz
:Hertz rdf:type owl:NamedIndividual ,
                :FrequencyUnit ;
       :hasAbbreviation "Hz" ;
       :hasSymbol "$1/s$" .


###  https://github.com/UTEP-Dynamic-Materials-Lab/SHPB_Toolkit/tree/main/ontology#Hexa8
:Hexa8 rdf:type owl:NamedIndividual ,
                <https://github.com/UTEP-Dynamic-Materials-Lab/SHPB_Toolkit/tree/main/ontology#3DElement> ;
       :hasDimension :ElementSize ;
       :hasAbbreviation "HEXA 8 Element" ;
       rdfs:comment "Represents the 8-node hexahedral solid element in LS-Dyna" ;
       :hasName "Fully Integrated 8 Point Hexa Element" .


###  https://github.com/UTEP-Dynamic-Materials-Lab/SHPB_Toolkit/tree/main/ontology#HighTemperature
:HighTemperature rdf:type owl:NamedIndividual ,
                          :TestTemperature ;
                 :hasAbbreviation "HT" ;
                 rdfs:comment "Indicates that the experiment was done using high temperature testing conditions." ;
                 :hasName "High Temparature Testing" .


###  https://github.com/UTEP-Dynamic-Materials-Lab/SHPB_Toolkit/tree/main/ontology#Inch
:Inch rdf:type owl:NamedIndividual ,
               :LengthUnit ;
      :hasAbbreviation "in" ;
      :hasSymbol "$in$" ;
      rdfs:comment "Inch, a unit of length in the English system." .


###  https://github.com/UTEP-Dynamic-Materials-Lab/SHPB_Toolkit/tree/main/ontology#InchPerSecond
:InchPerSecond rdf:type owl:NamedIndividual ,
                        :VelocityUnit ;
               :hasAbbreviation "in/s" ;
               :hasSymbol "$\\frac{in}{s}$" ;
               rdfs:comment "Inch per second, a unit of velocity in the English system." .


###  https://github.com/UTEP-Dynamic-Materials-Lab/SHPB_Toolkit/tree/main/ontology#IncidentBar
:IncidentBar rdf:type owl:NamedIndividual ,
                      :Bar ;
             :hasDimension :OriginalCrossSectionalArea ,
                           :OriginalDiameter ,
                           :OriginalLength ;
             :hasMaterial :SteelC350 ;
             :hasMechanicalProperty :Density ,
                                    :ElasticModulus ,
                                    :PoissonsRatio ,
                                    :WaveSpeed ;
             :hasLegendName "Incident Bar" ;
             rdfs:comment "Represents the Incident bar of a SHPB experimental setup. Each instance of this class must contain the assigned properties." .


###  https://github.com/UTEP-Dynamic-Materials-Lab/SHPB_Toolkit/tree/main/ontology#IncidentExtractedSignal
:IncidentExtractedSignal rdf:type owl:NamedIndividual ,
                                  :ExtractedSignal ;
                         :hasUnits :Unitless ;
                         rdfs:comment "Indicates the extracted signal from the incident bar, based on pulse duration. Used for SHPB analysis." .


###  https://github.com/UTEP-Dynamic-Materials-Lab/SHPB_Toolkit/tree/main/ontology#IncidentSensorSignal
:IncidentSensorSignal rdf:type owl:NamedIndividual ,
                               :SensorSignal ;
                      :hasUnits :MilliVolts ,
                                :Unitless ,
                                :Volts ;
                      :hasLegendName "Incident Signal" ;
                      rdfs:comment "Indicates the signal from the incident bar." .


###  https://github.com/UTEP-Dynamic-Materials-Lab/SHPB_Toolkit/tree/main/ontology#JohnsonCookModelSimplified
:JohnsonCookModelSimplified rdf:type owl:NamedIndividual ,
                                     :StrengthModel ;
                            :hasParameter :Density ,
                                          :ElasticModulus ,
                                          :HardeningExponent ,
                                          :HardeningModulus ,
                                          :PoissonsRatio ,
                                          :YieldStrength ;
                            :hasAbbreviation "JC Model" ;
                            rdfs:comment "Represents the Simplified JC Model, MAT 098, from LS-Dyna" ;
                            :hasName "Johnson-Cook Simplified Model" .


###  https://github.com/UTEP-Dynamic-Materials-Lab/SHPB_Toolkit/tree/main/ontology#Joule
:Joule rdf:type owl:NamedIndividual ,
                :EnergyUnit ;
       :hasAbbreviation "J" ;
       :hasSymbol "\\$J$" .


###  https://github.com/UTEP-Dynamic-Materials-Lab/SHPB_Toolkit/tree/main/ontology#KiloHertz
:KiloHertz rdf:type owl:NamedIndividual ,
                    :FrequencyUnit ;
           :hasAbbreviation "KHz" ;
           :hasSymbol "$KHz$" .


###  https://github.com/UTEP-Dynamic-Materials-Lab/SHPB_Toolkit/tree/main/ontology#KiloNewton
:KiloNewton rdf:type owl:NamedIndividual ,
                     :ForceUnit ;
            :hasAbbreviation "kN" ;
            :hasSymbol "$kN$" .


###  https://github.com/UTEP-Dynamic-Materials-Lab/SHPB_Toolkit/tree/main/ontology#KilogramPerCubicMeter
:KilogramPerCubicMeter rdf:type owl:NamedIndividual ,
                                :DensityUnit ;
                       :hasAbbreviation "Kg/m^3" ;
                       :hasSymbol "$\\frac{Kg}{m^3}$" ;
                       rdfs:comment "Kilogram per cubic meter, a unit of density." .


###  https://github.com/UTEP-Dynamic-Materials-Lab/SHPB_Toolkit/tree/main/ontology#KilogramPerCubicMillimeter
:KilogramPerCubicMillimeter rdf:type owl:NamedIndividual ,
                                     :DensityUnit ;
                            :hasAbbreviation "Kg/mm^3" ;
                            :hasSymbol "$\\frac{Kg}{mm^3}$" ;
                            rdfs:comment "Kilogram per cubic millimeter, a unit of density." .


###  https://github.com/UTEP-Dynamic-Materials-Lab/SHPB_Toolkit/tree/main/ontology#LABMode
:LABMode rdf:type owl:NamedIndividual ,
                  :TestMode ;
         :hasAbbreviation "LAB" ;
         rdfs:comment "Indicates that the experiment was done using physical testing conditions." ;
         :hasName "LAB Testing Conditions" .


###  https://github.com/UTEP-Dynamic-Materials-Lab/SHPB_Toolkit/tree/main/ontology#MachiningProcess
:MachiningProcess rdf:type owl:NamedIndividual ,
                           :SpecimenProcessing ;
                  :hasAbbreviation "Machined Specimen" ;
                  rdfs:comment "Refers to a specimen that was machined. Commonly used in SHPB testing." ;
                  :hasName "Machined Material" .


###  https://github.com/UTEP-Dynamic-Materials-Lab/SHPB_Toolkit/tree/main/ontology#MegaHertz
:MegaHertz rdf:type owl:NamedIndividual ,
                    :FrequencyUnit ;
           :hasAbbreviation "MHz" ;
           :hasSymbol "$MHz$" .


###  https://github.com/UTEP-Dynamic-Materials-Lab/SHPB_Toolkit/tree/main/ontology#Megapascal
:Megapascal rdf:type owl:NamedIndividual ,
                     :PressureUnit ;
            :hasAbbreviation "MPa" ;
            :hasSymbol "$\\text{MPa}$" ;
            rdfs:comment "Megapascal, a unit of pressure in the SI system." .


###  https://github.com/UTEP-Dynamic-Materials-Lab/SHPB_Toolkit/tree/main/ontology#Meter
:Meter rdf:type owl:NamedIndividual ,
                :LengthUnit ;
       :hasAbbreviation "m" ;
       :hasSymbol "$m$" ;
       rdfs:comment "Meter, a unit of length in the SI system." .


###  https://github.com/UTEP-Dynamic-Materials-Lab/SHPB_Toolkit/tree/main/ontology#MeterPerSecond
:MeterPerSecond rdf:type owl:NamedIndividual ,
                         :VelocityUnit ;
                :hasAbbreviation "m/s" ;
                :hasSymbol "$\\frac{m}{s}$" ;
                rdfs:comment "Meter per second, a unit of velocity in the SI system." .


###  https://github.com/UTEP-Dynamic-Materials-Lab/SHPB_Toolkit/tree/main/ontology#Micrometer
:Micrometer rdf:type owl:NamedIndividual ,
                     :LengthUnit ;
            :hasAbbreviation "$\\mu m$" ;
            :hasSymbol "$\\mu m$" ;
            rdfs:comment "Micrometer, a unit of length in the SI system." .


###  https://github.com/UTEP-Dynamic-Materials-Lab/SHPB_Toolkit/tree/main/ontology#Microsecond
:Microsecond rdf:type owl:NamedIndividual ,
                      :TimeUnit ;
             :hasAbbreviation "us" ;
             :hasSymbol "$\\mu s$" ;
             rdfs:comment "Microsecond, a unit of time in the SI system." .


###  https://github.com/UTEP-Dynamic-Materials-Lab/SHPB_Toolkit/tree/main/ontology#MilliOhms
:MilliOhms rdf:type owl:NamedIndividual ,
                    :ElectricalResistanceUnit ;
           :hasAbbreviation "mOhms" ;
           :hasSymbol "$m\\Omega$" .


###  https://github.com/UTEP-Dynamic-Materials-Lab/SHPB_Toolkit/tree/main/ontology#MilliVolts
:MilliVolts rdf:type owl:NamedIndividual ,
                     :ElectricPotentialUnit ;
            :hasAbbreviation "mV" ;
            :hasSymbol "$mV$" .


###  https://github.com/UTEP-Dynamic-Materials-Lab/SHPB_Toolkit/tree/main/ontology#Millijoule
:Millijoule rdf:type owl:NamedIndividual ,
                     :EnergyUnit ;
            :hasAbbreviation "mJ" ;
            :hasSymbol "\\$mJ$" .


###  https://github.com/UTEP-Dynamic-Materials-Lab/SHPB_Toolkit/tree/main/ontology#Millimeter
:Millimeter rdf:type owl:NamedIndividual ,
                     :LengthUnit ;
            :hasAbbreviation "mm" ;
            :hasSymbol "$mm$" ;
            rdfs:comment "Millimeter, a unit of length in the SI system." .


###  https://github.com/UTEP-Dynamic-Materials-Lab/SHPB_Toolkit/tree/main/ontology#MillimeterPerSecond
:MillimeterPerSecond rdf:type owl:NamedIndividual ,
                              :VelocityUnit ;
                     :hasAbbreviation "mm/s" ;
                     :hasSymbol "$\\frac{mm}{s}$" ;
                     rdfs:comment "Millimeter per second, a unit of velocity in the SI system." .


###  https://github.com/UTEP-Dynamic-Materials-Lab/SHPB_Toolkit/tree/main/ontology#Millisecond
:Millisecond rdf:type owl:NamedIndividual ,
                      :TimeUnit ;
             :hasAbbreviation "ms" ;
             :hasSymbol "$ms$" ;
             rdfs:comment "Millisecond, a unit of time in the SI system." .


###  https://github.com/UTEP-Dynamic-Materials-Lab/SHPB_Toolkit/tree/main/ontology#MomentumTrapEngaged
:MomentumTrapEngaged rdf:type owl:NamedIndividual ,
                              :MomentumTrap ;
                     :hasAbbreviation "Engaged" ;
                     rdfs:comment "Indicates that the momentum trap was engaged during the test." ;
                     :hasName "Momentum Trap Engaged" .


###  https://github.com/UTEP-Dynamic-Materials-Lab/SHPB_Toolkit/tree/main/ontology#MomentumTrapNotEngaged
:MomentumTrapNotEngaged rdf:type owl:NamedIndividual ,
                                 :MomentumTrap ;
                        :hasAbbreviation "Not Engaged" ;
                        rdfs:comment "Indicates that the momentum trap was not engaged during the test." ;
                        :hasName "Momentum Trap Not Engaged" .


###  https://github.com/UTEP-Dynamic-Materials-Lab/SHPB_Toolkit/tree/main/ontology#Monolithic
:Monolithic rdf:type owl:NamedIndividual ,
                     :Structure ;
            :hasAbbreviation "Mono" ;
            rdfs:comment "A monolithic structure is made from a single piece of material. In this context refered as fully dense structures of a single material alloy." ;
            :hasName "Monolithic" .


###  https://github.com/UTEP-Dynamic-Materials-Lab/SHPB_Toolkit/tree/main/ontology#Newton
:Newton rdf:type owl:NamedIndividual ,
                 :ForceUnit ;
        :hasAbbreviation "N" ;
        :hasSymbol "$N$" .


###  https://github.com/UTEP-Dynamic-Materials-Lab/SHPB_Toolkit/tree/main/ontology#NormalizingHT
:NormalizingHT rdf:type owl:NamedIndividual ;
               :hasAbbreviation "Normalized Alloy" ;
               rdfs:comment "Normalized Alloy" .


###  https://github.com/UTEP-Dynamic-Materials-Lab/SHPB_Toolkit/tree/main/ontology#Ohms
:Ohms rdf:type owl:NamedIndividual ,
               :ElectricalResistanceUnit ;
      :hasAbbreviation "Ohms" ;
      :hasSymbol "$\\Omega$" .


###  https://github.com/UTEP-Dynamic-Materials-Lab/SHPB_Toolkit/tree/main/ontology#OriginalCrossSectionalArea
:OriginalCrossSectionalArea rdf:type owl:NamedIndividual ,
                                     :Dimension ;
                            :hasUnits :SquareInches ,
                                      :SquareMeters ,
                                      :SquareMilimeters ;
                            :hasAbbreviation "Original Cross Section" ;
                            :hasName "Original Cross Sectional Area" .


###  https://github.com/UTEP-Dynamic-Materials-Lab/SHPB_Toolkit/tree/main/ontology#OriginalDiameter
:OriginalDiameter rdf:type owl:NamedIndividual ,
                           :Dimension ;
                  :hasUnits :Foot ,
                            :Inch ,
                            :Meter ,
                            :Micrometer ,
                            :Millimeter ;
                  :hasAbbreviation "Original Diameter" ;
                  :hasName "Original Diameter" .


###  https://github.com/UTEP-Dynamic-Materials-Lab/SHPB_Toolkit/tree/main/ontology#OriginalLength
:OriginalLength rdf:type owl:NamedIndividual ,
                         :Dimension ;
                :hasUnits :Foot ,
                          :Inch ,
                          :Meter ,
                          :Micrometer ,
                          :Millimeter ;
                :hasAbbreviation "Original Length" ;
                :hasName "Original Length" .


###  https://github.com/UTEP-Dynamic-Materials-Lab/SHPB_Toolkit/tree/main/ontology#ParticleVelocity
:ParticleVelocity rdf:type owl:NamedIndividual ,
                           :SeriesData ;
                  :hasUnits :MeterPerSecond ;
                  rdfs:comment "Represents particle velocity at specimen surface series data." .


###  https://github.com/UTEP-Dynamic-Materials-Lab/SHPB_Toolkit/tree/main/ontology#Pascal
:Pascal rdf:type owl:NamedIndividual ,
                 :PressureUnit ;
        :hasAbbreviation "Pa" ;
        :hasSymbol "$\\text{Pa}$" ;
        rdfs:comment "Pascal, a unit of pressure in the SI system." .


###  https://github.com/UTEP-Dynamic-Materials-Lab/SHPB_Toolkit/tree/main/ontology#PoissonsRatio
:PoissonsRatio rdf:type owl:NamedIndividual ,
                        :MechanicalProperty ;
               :hasUnits :Unitless ;
               :hasSymbol "$\\rho$" ;
               rdfs:comment "The ratio of transverse strain to axial strain in the elastic range." ;
               :hasName "Poisson's Ratio" .


###  https://github.com/UTEP-Dynamic-Materials-Lab/SHPB_Toolkit/tree/main/ontology#Pressure
:Pressure rdf:type owl:NamedIndividual ,
                   :Dimension ;
          :hasUnits :Gigapascal ,
                    :Megapascal ,
                    :Pascal ,
                    :Psi ;
          :hasAbbreviation "Pressure" ;
          :hasName "Pressure" .


###  https://github.com/UTEP-Dynamic-Materials-Lab/SHPB_Toolkit/tree/main/ontology#PrintCastProcess
:PrintCastProcess rdf:type owl:NamedIndividual ,
                           :SpecimenProcessing ;
                  :hasAbbreviation "Print Casted Specimen" ;
                  rdfs:comment "Refers to a specimen that was Print Casted. Commonly used in DynaMat Lab." ;
                  :hasName "Print Casting Composite" .


###  https://github.com/UTEP-Dynamic-Materials-Lab/SHPB_Toolkit/tree/main/ontology#Psi
:Psi rdf:type owl:NamedIndividual ,
              :PressureUnit ;
     :hasAbbreviation "psi" ;
     :hasSymbol "$\\text{psi}$" ;
     rdfs:comment "Pounds per square inch, a unit of pressure in the English system." .


###  https://github.com/UTEP-Dynamic-Materials-Lab/SHPB_Toolkit/tree/main/ontology#PulseDuration
:PulseDuration rdf:type owl:NamedIndividual ,
                        :PulseProperties ;
               :hasUnits :Millisecond ;
               rdfs:comment "Indicates the determined pulse duration of the test." .


###  https://github.com/UTEP-Dynamic-Materials-Lab/SHPB_Toolkit/tree/main/ontology#PulseLength
:PulseLength rdf:type owl:NamedIndividual ,
                      :PulseProperties ;
             :hasUnits :Millimeter ;
             rdfs:comment "Indicates the determined pulse length of the test." .


###  https://github.com/UTEP-Dynamic-Materials-Lab/SHPB_Toolkit/tree/main/ontology#PulseSpeed
:PulseSpeed rdf:type owl:NamedIndividual ,
                     :PulseProperties ;
            :hasUnits :MeterPerSecond ;
            rdfs:comment "Indicates the determined pulse speed of the test." .


###  https://github.com/UTEP-Dynamic-Materials-Lab/SHPB_Toolkit/tree/main/ontology#PulseStrainAmplitude
:PulseStrainAmplitude rdf:type owl:NamedIndividual ,
                               :PulseProperties ;
                      :hasUnits :Megapascal ;
                      rdfs:comment "Indicates the determined pulse strain amplitude of the test." .


###  https://github.com/UTEP-Dynamic-Materials-Lab/SHPB_Toolkit/tree/main/ontology#PulseStressAmplitude
:PulseStressAmplitude rdf:type owl:NamedIndividual ,
                               :PulseProperties ;
                      :hasUnits :Megapascal ;
                      rdfs:comment "Indicates the determined pulse stress amplitude of the test." .


###  https://github.com/UTEP-Dynamic-Materials-Lab/SHPB_Toolkit/tree/main/ontology#PulseTest
:PulseTest rdf:type owl:NamedIndividual ,
                    :TestType ;
           :hasAbbreviation "Pulse" ;
           rdfs:comment "A calibration SHPB test involving pulse evaluation without a specimen." ;
           :hasName "Pulse Test" .


###  https://github.com/UTEP-Dynamic-Materials-Lab/SHPB_Toolkit/tree/main/ontology#QuenchingHT
:QuenchingHT rdf:type owl:NamedIndividual ;
             :hasAbbreviation "Quenched Alloy" ;
             rdfs:comment "Quenched Alloy" .


###  https://github.com/UTEP-Dynamic-Materials-Lab/SHPB_Toolkit/tree/main/ontology#ReflectedExtractedSignal
:ReflectedExtractedSignal rdf:type owl:NamedIndividual ,
                                   :ExtractedSignal ;
                          :hasUnits :Volts ;
                          rdfs:comment "Indicates the reflected signal from the incident bar, based on pulse duration. Used for SHPB analysis." .


###  https://github.com/UTEP-Dynamic-Materials-Lab/SHPB_Toolkit/tree/main/ontology#Resistance
:Resistance rdf:type owl:NamedIndividual ,
                     :StrainGaugeProperties ;
            :hasUnits :MilliOhms ,
                      :Ohms ;
            rdfs:comment "Represents the resistance of the strain gauge in ohms." ;
            :hasName "Strain Gauge Resistance" .


###  https://github.com/UTEP-Dynamic-Materials-Lab/SHPB_Toolkit/tree/main/ontology#RoomTemperature
:RoomTemperature rdf:type owl:NamedIndividual ,
                          :TestTemperature ;
                 :hasAbbreviation "RT" ;
                 rdfs:comment "Indicates that the experiment was done using room temperature testing conditions." ;
                 :hasName "Room Temperature Testing" .


###  https://github.com/UTEP-Dynamic-Materials-Lab/SHPB_Toolkit/tree/main/ontology#SHPBExperiment
:SHPBExperiment rdf:type owl:NamedIndividual ,
                         :Experiment ;
                :hasAbbreviation "SHPB Test" ;
                :hasName "Split Hopkinson Pressure Bar Experiment" .


###  https://github.com/UTEP-Dynamic-Materials-Lab/SHPB_Toolkit/tree/main/ontology#SHPBSpecimen
:SHPBSpecimen rdf:type owl:NamedIndividual ,
                       :Specimen ;
              :hasDimension :DeformedCrossSectionalArea ,
                            :DeformedDiameter ,
                            :DeformedLength ,
                            :OriginalCrossSectionalArea ,
                            :OriginalDiameter ,
                            :OriginalLength ;
              :hasMechanicalProperty :Density ,
                                     :ElasticModulus ,
                                     :PoissonsRatio ;
              :hasShape :Cubic ,
                        :Cylindrical ;
              :hasStructure :GyroidLattice ,
                            :Monolithic ,
                            :SimpleCubicLattice ;
              rdfs:comment "Represents the instance of SHPB Experiments. Each test must have the following values for each specimen" ;
              :hasName "FEA Specimen" .


###  https://github.com/UTEP-Dynamic-Materials-Lab/SHPB_Toolkit/tree/main/ontology#SHPBStrainGauge
:SHPBStrainGauge rdf:type owl:NamedIndividual ,
                          :StrainGauge ;
                 :hasDimension :StrainGaugeDistance ;
                 :hasStrainGaugeProperty :CalibrationResistance ,
                                         :CalibrationVoltage ,
                                         :GaugeFactor ,
                                         :Resistance ;
                 :hasAbbreviation "SG" ;
                 :hasName "Strain Guage for Split Hopkinson Pressure Bar Testing" .


###  https://github.com/UTEP-Dynamic-Materials-Lab/SHPB_Toolkit/tree/main/ontology#SS316
:SS316 rdf:type owl:NamedIndividual ,
                :SteelAlloy ;
       :hasAbbreviation "SS316" ;
       :hasLegendName "SS316 Alloy" ;
       :hasName "Stainless Steel 316 Alloy" .


###  https://github.com/UTEP-Dynamic-Materials-Lab/SHPB_Toolkit/tree/main/ontology#SS316A356_Composite
:SS316A356_Composite rdf:type owl:NamedIndividual ,
                              :CompositeMaterial ;
                     :hasAbbreviation "SS316A356" ;
                     :hasLegendName "SS 316 - Al 356 Composite" ;
                     :hasName "Stainless 316 - A356 Composite" .


###  https://github.com/UTEP-Dynamic-Materials-Lab/SHPB_Toolkit/tree/main/ontology#Second
:Second rdf:type owl:NamedIndividual ,
                 :TimeUnit ;
        :hasAbbreviation "s" ;
        :hasSymbol "$s$" ;
        rdfs:comment "Second, a unit of time in the SI system." .


###  https://github.com/UTEP-Dynamic-Materials-Lab/SHPB_Toolkit/tree/main/ontology#SimpleCubicLattice
:SimpleCubicLattice rdf:type owl:NamedIndividual ,
                             :Structure ;
                    :hasAbbreviation "SC" ;
                    rdfs:comment "A simple cubic structure is a crystal structure with a cube-shaped unit cell. Represents the simple cubic bravais lattice used in material science." ;
                    :hasName "Simple Cubic Lattice" .


###  https://github.com/UTEP-Dynamic-Materials-Lab/SHPB_Toolkit/tree/main/ontology#SolutionHT
:SolutionHT rdf:type owl:NamedIndividual ;
            :hasAbbreviation "Solution Hardened Alloy" ;
            rdfs:comment "Solution Hardened Alloy" .


###  https://github.com/UTEP-Dynamic-Materials-Lab/SHPB_Toolkit/tree/main/ontology#SpecimenTest
:SpecimenTest rdf:type owl:NamedIndividual ,
                       :TestType ;
              :hasAbbreviation "Specimen" ;
              rdfs:comment "A test involving a specimen to evaluate its mechanical behavior." ;
              :hasName "Specimen Test" .


###  https://github.com/UTEP-Dynamic-Materials-Lab/SHPB_Toolkit/tree/main/ontology#SquareInches
:SquareInches rdf:type owl:NamedIndividual ,
                       :AreaUnit ;
              :hasAbbreviation "in^2" ;
              :hasSymbol "$in^2$" .


###  https://github.com/UTEP-Dynamic-Materials-Lab/SHPB_Toolkit/tree/main/ontology#SquareMeters
:SquareMeters rdf:type owl:NamedIndividual ,
                       :AreaUnit ;
              :hasAbbreviation "m^2" ;
              :hasSymbol "$m^2$" .


###  https://github.com/UTEP-Dynamic-Materials-Lab/SHPB_Toolkit/tree/main/ontology#SquareMilimeters
:SquareMilimeters rdf:type owl:NamedIndividual ,
                           :AreaUnit ;
                  :hasAbbreviation "mm^2" ;
                  :hasSymbol "$mm^2$" .


###  https://github.com/UTEP-Dynamic-Materials-Lab/SHPB_Toolkit/tree/main/ontology#Steel1018
:Steel1018 rdf:type owl:NamedIndividual ,
                    :SteelAlloy ;
           :hasAbbreviation "ST1018" ;
           :hasLegendName "ST1018 Alloy" ;
           :hasName "Steel 1018 Alloy" .


###  https://github.com/UTEP-Dynamic-Materials-Lab/SHPB_Toolkit/tree/main/ontology#SteelC350
:SteelC350 rdf:type owl:NamedIndividual ,
                    :SteelAlloy ;
           :hasAbbreviation "STC350" ;
           :hasLegendName "STC350 Alloy" ;
           :hasName "Steel C350 Alloy" .


###  https://github.com/UTEP-Dynamic-Materials-Lab/SHPB_Toolkit/tree/main/ontology#StrainEnergy
:StrainEnergy rdf:type owl:NamedIndividual ,
                       :SeriesData ;
              rdfs:comment "Represents strain energy series data." .


###  https://github.com/UTEP-Dynamic-Materials-Lab/SHPB_Toolkit/tree/main/ontology#StrainGaugeDistance
:StrainGaugeDistance rdf:type owl:NamedIndividual ,
                              :Dimension ;
                     :hasUnits :Foot ,
                               :Inch ,
                               :Meter ,
                               :Micrometer ,
                               :Millimeter ;
                     :hasAbbreviation "Strain Gauge Dist" ;
                     :hasName "Strain Gauge Distance" .


###  https://github.com/UTEP-Dynamic-Materials-Lab/SHPB_Toolkit/tree/main/ontology#StrainRateCoefficient
:StrainRateCoefficient rdf:type owl:NamedIndividual ,
                                :MechanicalProperty ;
                       :hasSymbol "$C$" ;
                       rdfs:comment "Describes the material's strain rate sensitivity. Commonly used in constitutive equations under high-loading rates." ,
                                    "Represents the parameter \"c\" in LS-Dyna Model" ;
                       :hasName "Strain Rate Coefficient" .


###  https://github.com/UTEP-Dynamic-Materials-Lab/SHPB_Toolkit/tree/main/ontology#StrikerBar
:StrikerBar rdf:type owl:NamedIndividual ,
                     :Bar ;
            :hasDimension :OriginalCrossSectionalArea ,
                          :OriginalDiameter ,
                          :OriginalLength ;
            :hasMaterial :SteelC350 ;
            :hasMechanicalProperty :Density ,
                                   :ElasticModulus ,
                                   :PoissonsRatio ,
                                   :WaveSpeed ;
            :hasLegendName "Striker Bar" ;
            rdfs:comment "Represents the striker bar of a SHPB experimental setup. Each instance of this class must contain the assigned properties." .


###  https://github.com/UTEP-Dynamic-Materials-Lab/SHPB_Toolkit/tree/main/ontology#SurfaceForce
:SurfaceForce rdf:type owl:NamedIndividual ,
                       :SeriesData .


###  https://github.com/UTEP-Dynamic-Materials-Lab/SHPB_Toolkit/tree/main/ontology#TemperatureExtractedSignal
:TemperatureExtractedSignal rdf:type owl:NamedIndividual ,
                                     :ExtractedSignal ;
                            :hasUnits :DegreesCelsius ;
                            rdfs:comment "Indicates the extracted signal from the temperature sensor, based on pulse duration. Used for SHPB analysis." .


###  https://github.com/UTEP-Dynamic-Materials-Lab/SHPB_Toolkit/tree/main/ontology#TemperatureSensorSignal
:TemperatureSensorSignal rdf:type owl:NamedIndividual ,
                                  :SensorSignal ;
                         :hasUnits :DegreesCelsius ,
                                   :DegressFahrenheit ;
                         :hasLegendName "Temperature Signal" ;
                         rdfs:comment "Indicates the signal from the temperature sensor." .


###  https://github.com/UTEP-Dynamic-Materials-Lab/SHPB_Toolkit/tree/main/ontology#TemperedHT
:TemperedHT rdf:type owl:NamedIndividual ;
            :hasAbbreviation "Tempered Alloy" ;
            rdfs:comment "Tempered Alloy" .


###  https://github.com/UTEP-Dynamic-Materials-Lab/SHPB_Toolkit/tree/main/ontology#ThermalSofteningCoefficient
:ThermalSofteningCoefficient rdf:type owl:NamedIndividual ,
                                      :MechanicalProperty ;
                             rdfs:comment "Describes the coefficient of thermal softening. Describes how the material's yield stress decreases as the temperature increases. Commonly used to model the behavior under high-rate loading." ;
                             :hasName "Thermal Softening Coefficient" .


###  https://github.com/UTEP-Dynamic-Materials-Lab/SHPB_Toolkit/tree/main/ontology#TimeExtractedSignal
:TimeExtractedSignal rdf:type owl:NamedIndividual ,
                              :ExtractedSignal ;
                     :hasUnits :Millisecond ;
                     rdfs:comment "Represents the pulse duration. Used for SHPB analysis." .


###  https://github.com/UTEP-Dynamic-Materials-Lab/SHPB_Toolkit/tree/main/ontology#TimeSensorSignal
:TimeSensorSignal rdf:type owl:NamedIndividual ,
                           :SensorSignal ;
                  :hasUnits :Microsecond ,
                            :Millisecond ,
                            :Second ;
                  :hasLegendName "Time Signal" ;
                  rdfs:comment "Indicates the time signal collected." .


###  https://github.com/UTEP-Dynamic-Materials-Lab/SHPB_Toolkit/tree/main/ontology#TransmittedBar
:TransmittedBar rdf:type owl:NamedIndividual ,
                         :Bar ;
                :hasDimension :OriginalCrossSectionalArea ,
                              :OriginalDiameter ,
                              :OriginalLength ;
                :hasMaterial :SteelC350 ;
                :hasMechanicalProperty :Density ,
                                       :ElasticModulus ,
                                       :PoissonsRatio ,
                                       :WaveSpeed ;
                :hasLegendName "Transmitted Bar" ;
                rdfs:comment "Represents the transmitted bar of a SHPB experimental setup. Each instance of this class must contain the assigned properties." .


###  https://github.com/UTEP-Dynamic-Materials-Lab/SHPB_Toolkit/tree/main/ontology#TransmittedExtractedSignal
:TransmittedExtractedSignal rdf:type owl:NamedIndividual ,
                                     :ExtractedSignal ;
                            :hasUnits :Unitless ;
                            rdfs:comment "Indicates the extracted signal from the transmitted bar, based on pulse duration. Used for SHPB analysis." .


###  https://github.com/UTEP-Dynamic-Materials-Lab/SHPB_Toolkit/tree/main/ontology#TransmittedSensorSignal
:TransmittedSensorSignal rdf:type owl:NamedIndividual ,
                                  :SensorSignal ;
                         :hasUnits :MilliVolts ,
                                   :Unitless ,
                                   :Volts ;
                         :hasLegendName "Transmitted Signal" ;
                         rdfs:comment "Indicates the signal from the transmitted bar." .


###  https://github.com/UTEP-Dynamic-Materials-Lab/SHPB_Toolkit/tree/main/ontology#TrueStrain
:TrueStrain rdf:type owl:NamedIndividual ,
                     :SeriesData ;
            :hasSymbol "$\\varepsilon_T$" ;
            rdfs:comment "Represents true strain series data." ;
            :hasName "True Strain" .


###  https://github.com/UTEP-Dynamic-Materials-Lab/SHPB_Toolkit/tree/main/ontology#TrueStress
:TrueStress rdf:type owl:NamedIndividual ,
                     :SeriesData ;
            :hasSymbol "$\\sigma_T$" ;
            rdfs:comment "Represents true stress series data." ;
            :hasName "True Stress" .


###  https://github.com/UTEP-Dynamic-Materials-Lab/SHPB_Toolkit/tree/main/ontology#Unitless
:Unitless rdf:type owl:NamedIndividual ,
                   :UnitlessUnit ;
          :hasAbbreviation "Unitless" ;
          :hasSymbol "" .


###  https://github.com/UTEP-Dynamic-Materials-Lab/SHPB_Toolkit/tree/main/ontology#Velocity
:Velocity rdf:type owl:NamedIndividual ,
                   :Dimension ;
          :hasUnits :InchPerSecond ,
                    :MeterPerSecond ;
          :hasAbbreviation "Velocity" ;
          :hasName "Velocity" .


###  https://github.com/UTEP-Dynamic-Materials-Lab/SHPB_Toolkit/tree/main/ontology#Volts
:Volts rdf:type owl:NamedIndividual ,
                :ElectricPotentialUnit ;
       :hasAbbreviation "V" ;
       :hasSymbol "$V$" .


###  https://github.com/UTEP-Dynamic-Materials-Lab/SHPB_Toolkit/tree/main/ontology#WaveSpeed
:WaveSpeed rdf:type owl:NamedIndividual ,
                    :MechanicalProperty ;
           :hasUnits :InchPerSecond ,
                     :MeterPerSecond ;
           rdfs:comment "Speed of stress waves through the material during testing." ;
           :hasName "Wave Speed" .


###  https://github.com/UTEP-Dynamic-Materials-Lab/SHPB_Toolkit/tree/main/ontology#YieldStrength
:YieldStrength rdf:type owl:NamedIndividual ,
                        :MechanicalProperty ;
               :hasUnits :Gigapascal ,
                         :Megapascal ,
                         :Pascal ,
                         :Psi ;
               :hasSymbol "$\\sigma_Y$" ;
               rdfs:comment "Initial yield strength of the material." ;
               :hasName "Yield Strength" .


###  https://github.com/UTEP-Dynamic-Materials-Lab/SHPB_Toolkit/tree/main/ontology#3DPrintingProcess
<https://github.com/UTEP-Dynamic-Materials-Lab/SHPB_Toolkit/tree/main/ontology#3DPrintingProcess> rdf:type owl:NamedIndividual ,
                                                                                                           :SpecimenProcessing ;
                                                                                                  :hasAbbreviation "3D Printed Specimen" ;
                                                                                                  rdfs:comment "Refers to a specimen that was 3D Printed. Commonly used in SHPB testing" ;
                                                                                                  :hasName "3D Printed Material" .


#################################################################
#    Annotations
#################################################################

:hasName rdfs:comment "Full name of the user." .


###  Generated by the OWL API (version 4.5.29.2024-05-13T12:11:03Z) https://github.com/owlcs/owlapi
