@prefix : <http://www.semanticweb.org/ecazares3/ontologies/DynaMat_SHPB#> .
@prefix owl: <http://www.w3.org/2002/07/owl#> .
@prefix rdf: <http://www.w3.org/1999/02/22-rdf-syntax-ns#> .
@prefix xml: <http://www.w3.org/XML/1998/namespace> .
@prefix xsd: <http://www.w3.org/2001/XMLSchema#> .
@prefix rdfs: <http://www.w3.org/2000/01/rdf-schema#> .
@base <http://www.semanticweb.org/ecazares3/ontologies/DynaMat_SHPB#> .

<http://www.semanticweb.org/ecazares3/ontologies/DynaMat_SHPB> rdf:type owl:Ontology .

#################################################################
#    Datatypes
#################################################################

###  http://www.w3.org/2001/XMLSchema#date
xsd:date rdf:type rdfs:Datatype .


#################################################################
#    Object Properties
#################################################################

###  http://www.semanticweb.org/ecazares3/ontologies/DynaMat_SHPB#hasDeterminedTimeSeries
:hasDeterminedTimeSeries rdf:type owl:ObjectProperty ;
                         rdfs:domain :SecondaryData ;
                         rdfs:range :SeriesType ;
                         rdfs:comment "Links secondary data to extracted related series, such as stress-strain curves." .


###  http://www.semanticweb.org/ecazares3/ontologies/DynaMat_SHPB#hasExtractedPulse
:hasExtractedPulse rdf:type owl:ObjectProperty ;
                   rdfs:domain :SecondaryData ;
                   rdfs:range :SignalType ;
                   rdfs:comment "Links secondary data to extracted time-series signals, such as strain." .


###  http://www.semanticweb.org/ecazares3/ontologies/DynaMat_SHPB#hasMaterial
:hasMaterial rdf:type owl:ObjectProperty ;
             rdfs:domain [ rdf:type owl:Class ;
                           owl:unionOf ( :Bar
                                         :Specimen
                                       )
                         ] ;
             rdfs:range :Material ;
             rdfs:comment "Links bars or specimens to their associated material." .


:hasMechanicalProperty rdf:type owl:ObjectProperty ;
                       rdfs:domain [ owl:unionOf ( :MechanicalProperty :SecondaryData ) ] ;
                       rdfs:range [ owl:unionOf ( :Bar :Specimen :DeterminedMechanicalProperty ) ] ;
                       rdfs:comment "Links a specific mechanical property to a Bar, Specimen, or a determined property in SecondaryData." .


###  http://www.semanticweb.org/ecazares3/ontologies/DynaMat_SHPB#hasMomentumTrapCondition
:hasMomentumTrapCondition rdf:type owl:ObjectProperty ;
                          rdfs:domain :Metadata ;
                          rdfs:range :TestingConditions ;
                          rdfs:comment "Links metadata to test configurations, such as momentum trap engagement." .


###  http://www.semanticweb.org/ecazares3/ontologies/DynaMat_SHPB#hasParameter
:hasParameter rdf:type owl:ObjectProperty ;
              rdfs:domain :StrengthModel ;
              rdfs:range :Parameter ;
              rdfs:comment "Links a strength model to its parameters." .


###  http://www.semanticweb.org/ecazares3/ontologies/DynaMat_SHPB#hasSensorSignal
:hasSensorSignal rdf:type owl:ObjectProperty ;
                 rdfs:domain :PrimaryData ;
                 rdfs:range :SignalType ;
                 rdfs:comment "Links primary data to specific time-series signals, such as strain." .


###  http://www.semanticweb.org/ecazares3/ontologies/DynaMat_SHPB#hasSeriesType
:hasSeriesType rdf:type owl:ObjectProperty ;
               rdfs:domain :SeriesData ;
               rdfs:range :SeriesType ;
               rdfs:comment "Links a data series to its series type using controlled vocabulary." .


###  http://www.semanticweb.org/ecazares3/ontologies/DynaMat_SHPB#hasSignalType
:hasSignalType rdf:type owl:ObjectProperty ;
               rdfs:domain :ExtractedSignal ,
                           :SensorSignal ;
               rdfs:range :SignalType ;
               rdfs:comment "Links a sensor signal to its signal type using controlled vocabulary." .


###  http://www.semanticweb.org/ecazares3/ontologies/DynaMat_SHPB#hasSpecimen
:hasSpecimen rdf:type owl:ObjectProperty ;
             rdfs:domain :Metadata ;
             rdfs:range :Specimen ;
             rdfs:comment "Links metadata to the specimen details." .

###  http://www.semanticweb.org/ecazares3/ontologies/DynaMat_SHPB#hasStrainGaugeProperty
:hasStrainGaugeProperty rdf:type owl:ObjectProperty ;
                        rdfs:domain :TestingConditions ;
                        rdfs:range :StrainGaugeProperties ;
                        rdfs:comment "Links laboratory metadata to strain gauge properties." .


###  http://www.semanticweb.org/ecazares3/ontologies/DynaMat_SHPB#hasTestType
:hasTestType rdf:type owl:ObjectProperty ;
             rdfs:domain :Metadata ;
             rdfs:range :TestType ;
             rdfs:comment "Links test metadata to its associated test type, such as pulse or specimen testing." .


###  http://www.semanticweb.org/ecazares3/ontologies/DynaMat_SHPB#hasTestingConditions
:hasTestingConditions rdf:type owl:ObjectProperty ;
                      rdfs:domain :Metadata ;
                      rdfs:range :TestingConditions ;
                      rdfs:comment "Specifies the type of setup used, such as lab-based or simulation-based." .


###  http://www.semanticweb.org/ecazares3/ontologies/DynaMat_SHPB#hasTime
:hasTime rdf:type owl:ObjectProperty ;
         rdfs:domain [ owl:unionOf ( :PrimaryData :SecondaryData ) ] ;
         rdfs:comment "Links data to extracted time signals." .


#################################################################
#    Data properties
#################################################################

###  http://www.semanticweb.org/ecazares3/ontologies/DynaMat_SHPB#hasAffiliation
:hasAffiliation rdf:type owl:DatatypeProperty ;
                rdfs:domain :Laboratory ;
                rdfs:range xsd:string ;
                rdfs:comment "Specifies the institution or organization the laboratory is affiliated with." .


###  http://www.semanticweb.org/ecazares3/ontologies/DynaMat_SHPB#hasChemicalComposition
:hasChemicalComposition rdf:type owl:DatatypeProperty ;
                        rdfs:domain :Material ;
                        rdfs:range xsd:string ;
                        rdfs:comment "Specifies the chemical composition of the specimen." .


###  http://www.semanticweb.org/ecazares3/ontologies/DynaMat_SHPB#hasCrossSection
:hasCrossSection rdf:type owl:DatatypeProperty ;
                 rdfs:domain [ rdf:type owl:Class ;
                               owl:unionOf ( :Bar
                                             :Specimen
                                           )
                             ] ;
                 rdfs:range xsd:float ;
                 rdfs:comment "Specifies the cross-sectional area in square meters." .


:hasDataAcquisitionRate rdf:type owl:DatatypeProperty ;
                        rdfs:domain :Metadata ;
                        rdfs:range xsd:float ;
                        rdfs:comment "Specifies the data acquisition rate, such as sampling frequency in Hz." .

###  http://www.semanticweb.org/ecazares3/ontologies/DynaMat_SHPB#hasEncoding
:hasEncoding rdf:type owl:DatatypeProperty ;
             rdfs:range xsd:string ;
             rdfs:comment "Specifies the encoding used for storing the data, such as 'Base64'." .


###  http://www.semanticweb.org/ecazares3/ontologies/DynaMat_SHPB#hasLength
:hasLength rdf:type owl:DatatypeProperty ;
           rdfs:domain [ rdf:type owl:Class ;
                         owl:unionOf ( :Bar
                                       :Specimen
                                     )
                       ] ;
           rdfs:range xsd:float ;
           rdfs:comment "Specifies the length in meters." .


###  http://www.semanticweb.org/ecazares3/ontologies/DynaMat_SHPB#hasLocation
:hasLocation rdf:type owl:DatatypeProperty ;
             rdfs:domain :Laboratory ;
             rdfs:range xsd:string ;
             rdfs:comment "Specifies the location of the laboratory, e.g., Building A, Room 12." .


###  http://www.semanticweb.org/ecazares3/ontologies/DynaMat_SHPB#hasMaterialClass
:hasMaterialClass rdf:type owl:DatatypeProperty ;
                  rdfs:domain :Material ;
                  rdfs:range xsd:string ;
                  rdfs:comment "Specifies the material class of the specimen." .


###  http://www.semanticweb.org/ecazares3/ontologies/DynaMat_SHPB#hasMaterialProcessing
:hasMaterialProcessing rdf:type owl:DatatypeProperty ;
                       rdfs:domain :Material ;
                       rdfs:range xsd:string ;
                       rdfs:comment "Specifies the processing of the specimen material." .


###  http://www.semanticweb.org/ecazares3/ontologies/DynaMat_SHPB#hasName
:hasName rdf:type owl:DatatypeProperty ;
         rdfs:range xsd:string ;
         rdfs:comment "Gives a human-readable name for the series or scalar value." .


###  http://www.semanticweb.org/ecazares3/ontologies/DynaMat_SHPB#hasShape
:hasShape rdf:type owl:DatatypeProperty ;
          rdfs:domain :Specimen ;
          rdfs:range xsd:string ;
          rdfs:comment "Specifies the shape of the specimen, e.g., cylindrical or rectangular." .


###  http://www.semanticweb.org/ecazares3/ontologies/DynaMat_SHPB#hasSize
:hasSize rdf:type owl:DatatypeProperty ;
         rdfs:range xsd:integer ;
         rdfs:comment "Indicates the size of the dataset, such as the number of points in a series." .


###  http://www.semanticweb.org/ecazares3/ontologies/DynaMat_SHPB#hasStructure
:hasStructure rdf:type owl:DatatypeProperty ;
              rdfs:domain :Specimen ;
              rdfs:range xsd:string ;
              rdfs:comment "Specifies the structure of the specimen, e.g., amorphous, crystalline, or composite." .


###  http://www.semanticweb.org/ecazares3/ontologies/DynaMat_SHPB#hasSupervisor
:hasSupervisor rdf:type owl:DatatypeProperty ;
               rdfs:domain :Laboratory ;
               rdfs:range xsd:string ;
               rdfs:comment "Specifies the name of the test supervisor." .


###  http://www.semanticweb.org/ecazares3/ontologies/DynaMat_SHPB#hasSymbol
:hasSymbol rdf:type owl:DatatypeProperty ;
           rdfs:range xsd:string ;
           rdfs:comment "Provides the LaTeX symbol for use in plotting or labeling." .


###  http://www.semanticweb.org/ecazares3/ontologies/DynaMat_SHPB#hasTestDate
:hasTestDate rdf:type owl:DatatypeProperty ;
             rdfs:domain :Metadata ;
             rdfs:range xsd:date ;
             rdfs:comment "Specifies the date the test was performed." .


###  http://www.semanticweb.org/ecazares3/ontologies/DynaMat_SHPB#hasTestName
:hasTestName rdf:type owl:DatatypeProperty ;
             rdfs:domain :Metadata ;
             rdfs:range xsd:string ;
             rdfs:comment "Specifies the name of the test." .


###  http://www.semanticweb.org/ecazares3/ontologies/DynaMat_SHPB#hasUnits
:hasUnits rdf:type owl:DatatypeProperty ;
          rdfs:range xsd:string ;
          rdfs:comment "Specifies the physical units of a data series or scalar value." .


###  http://www.semanticweb.org/ecazares3/ontologies/DynaMat_SHPB#hasUser
:hasUser rdf:type owl:DatatypeProperty ;
         rdfs:domain :Metadata ;
         rdfs:range xsd:string ;
         rdfs:comment "Specifies the user who performed the test." .


###  http://www.semanticweb.org/ecazares3/ontologies/DynaMat_SHPB#hasValue
:hasValue rdf:type owl:DatatypeProperty ;
          rdfs:range xsd:float ;
          rdfs:comment "Stores the numerical value of a scalar property, such as UTS." .


#################################################################
#    Classes
#################################################################

###  http://www.semanticweb.org/ecazares3/ontologies/DynaMat_SHPB#Bar
:Bar rdf:type owl:Class ;
     rdfs:subClassOf :TestingConditions ;
     rdfs:comment "Defines the generic class for bar properties." .


###  http://www.semanticweb.org/ecazares3/ontologies/DynaMat_SHPB#DeterminedMechanicalProperty
:DeterminedMechanicalProperty rdf:type owl:Class ;
                              rdfs:subClassOf :SecondaryData ;
                              rdfs:comment "Represents the subsection of determined mechanical properties from test." .


###  http://www.semanticweb.org/ecazares3/ontologies/DynaMat_SHPB#ExtractedSignal
:ExtractedSignal rdf:type owl:Class ;
                 rdfs:subClassOf :SecondaryData ;
                 rdfs:comment "Represents the determined particle velocity at a surface of the specimen." .


###  http://www.semanticweb.org/ecazares3/ontologies/DynaMat_SHPB#FEMetadata
:FEMetadata rdf:type owl:Class ;
            rdfs:subClassOf :Bar ,
                            :Specimen ;
            rdfs:comment "Metadata specific to finite element-based simulations." .


###  http://www.semanticweb.org/ecazares3/ontologies/DynaMat_SHPB#Laboratory
:Laboratory rdf:type owl:Class ;
            rdfs:subClassOf :Metadata ;
            rdfs:comment "Describes the Laboratory." .


###  http://www.semanticweb.org/ecazares3/ontologies/DynaMat_SHPB#Material
:Material rdf:type owl:Class ;
          rdfs:comment "Represents a generic material, including mandatory composition and class attributes." .


###  http://www.semanticweb.org/ecazares3/ontologies/DynaMat_SHPB#MechanicalProperty
:MechanicalProperty rdf:type owl:Class ;
                    rdfs:subClassOf :Bar ,
                                    :Specimen ;
                    rdfs:comment "Describes the density property of a component." ,
                                 "Represents a mechanical property that characterizes the material behavior, such as elastic modulus or density." .


###  http://www.semanticweb.org/ecazares3/ontologies/DynaMat_SHPB#Metadata
:Metadata rdf:type owl:Class ;
          rdfs:comment "Captures general metadata about the test, including conditions and setup." .


###  http://www.semanticweb.org/ecazares3/ontologies/DynaMat_SHPB#MomentumTrap
:MomentumTrap rdf:type owl:Class ;
              rdfs:subClassOf :TestingConditions ;
              rdfs:comment "Striker impact velocity." .


###  http://www.semanticweb.org/ecazares3/ontologies/DynaMat_SHPB#Parameter
:Parameter rdf:type owl:Class ;
           rdfs:subClassOf :StrengthModel ;
           rdfs:comment "Represents a parameter within a strength model, including its value and units." .


###  http://www.semanticweb.org/ecazares3/ontologies/DynaMat_SHPB#PrimaryData
:PrimaryData rdf:type owl:Class ;
             rdfs:comment "Represents raw data directly collected during the SHPB test, including strain gauge signals." .


###  http://www.semanticweb.org/ecazares3/ontologies/DynaMat_SHPB#SecondaryData
:SecondaryData rdf:type owl:Class ;
               rdfs:comment "Represents processed data and determined mechanical properties, including series and single-value properties." .


###  http://www.semanticweb.org/ecazares3/ontologies/DynaMat_SHPB#SensorSignal
:SensorSignal rdf:type owl:Class ;
              rdfs:subClassOf :PrimaryData ;
              rdfs:comment "Represents a generic signal from a sensor." .


###  http://www.semanticweb.org/ecazares3/ontologies/DynaMat_SHPB#SeriesData
:SeriesData rdf:type owl:Class ;
            rdfs:subClassOf :SecondaryData ;
            rdfs:comment "Represents a generic data series, such as stress or strain." .


###  http://www.semanticweb.org/ecazares3/ontologies/DynaMat_SHPB#SeriesType
:SeriesType rdf:type owl:Class ;
            rdfs:comment "Represents a controlled vocabulary for series types." .


###  http://www.semanticweb.org/ecazares3/ontologies/DynaMat_SHPB#SignalType
:SignalType rdf:type owl:Class ;
            rdfs:comment "Represents a controlled vocabulary for signal types." .


###  http://www.semanticweb.org/ecazares3/ontologies/DynaMat_SHPB#Specimen
:Specimen rdf:type owl:Class ;
          rdfs:subClassOf :Metadata ;
          rdfs:comment "Describes the specimen tested, including its material and geometry." .


###  http://www.semanticweb.org/ecazares3/ontologies/DynaMat_SHPB#StrainGaugeFactorType
:StrainGaugeFactorType rdf:type owl:Class ;
                       rdfs:comment "Controlled vocabulary for types of strain gauge factors." .


###  http://www.semanticweb.org/ecazares3/ontologies/DynaMat_SHPB#StrainGaugeProperties
:StrainGaugeProperties rdf:type owl:Class ;
                       rdfs:subClassOf :TestingConditions ;
                       rdfs:comment "Captures all properties related to strain gauge calibration." .


###  http://www.semanticweb.org/ecazares3/ontologies/DynaMat_SHPB#StrengthModel
:StrengthModel rdf:type owl:Class ;
               rdfs:subClassOf :FEMetadata ;
               rdfs:comment "Represents the strength model used in finite element analysis." .


###  http://www.semanticweb.org/ecazares3/ontologies/DynaMat_SHPB#TestType
:TestType rdf:type owl:Class ;
          rdfs:comment "Represents the type of test conducted, such as pulse calibration or specimen testing." .


###  http://www.semanticweb.org/ecazares3/ontologies/DynaMat_SHPB#TestingConditions
:TestingConditions rdf:type owl:Class ;
                   rdfs:subClassOf :Metadata ;
                   rdfs:comment "Metadata specific to Testing Conditions." .


###  http://www.semanticweb.org/ecazares3/ontologies/DynaMat_SHPB#TimeSeries
:TimeSeries rdf:type owl:Class ;
            rdfs:subClassOf :PrimaryData ;
            rdfs:comment "Represents the time signal from the data acquisition system." .


#################################################################
#    Individuals
#################################################################

###  http://www.semanticweb.org/ecazares3/ontologies/DynaMat_SHPB#AbsorbedEnergy
:AbsorbedEnergy rdf:type owl:NamedIndividual ,
                         :SeriesType ;
                rdfs:comment "Represents absorbed energy." .


###  http://www.semanticweb.org/ecazares3/ontologies/DynaMat_SHPB#CalibrationResistance
:CalibrationResistance rdf:type owl:NamedIndividual ,
                                :StrainGaugeFactorType ;
                       rdfs:comment "Represents the calibration resistance of the strain gauge in ohms." .


###  http://www.semanticweb.org/ecazares3/ontologies/DynaMat_SHPB#CalibrationVoltage
:CalibrationVoltage rdf:type owl:NamedIndividual ,
                             :StrainGaugeFactorType ;
                    rdfs:comment "Represents the calibration voltage of the strain gauge in volts." .


###  http://www.semanticweb.org/ecazares3/ontologies/DynaMat_SHPB#Density
:Density rdf:type owl:NamedIndividual ,
                  :MechanicalProperty ;
         rdfs:comment "The mass per unit volume of the material." .


###  http://www.semanticweb.org/ecazares3/ontologies/DynaMat_SHPB#ElasticModulus
:ElasticModulus rdf:type owl:NamedIndividual ,
                         :MechanicalProperty ;
                rdfs:comment "Represents the stiffness of the material in the elastic range." .


###  http://www.semanticweb.org/ecazares3/ontologies/DynaMat_SHPB#EngineeringStrain
:EngineeringStrain rdf:type owl:NamedIndividual ,
                            :SeriesType ;
                   rdfs:comment "Represents engineering strain." .


###  http://www.semanticweb.org/ecazares3/ontologies/DynaMat_SHPB#EngineeringStrainRate
:EngineeringStrainRate rdf:type owl:NamedIndividual ,
                                :SeriesType ;
                       rdfs:comment "Represents engineering strain rate." .


###  http://www.semanticweb.org/ecazares3/ontologies/DynaMat_SHPB#EngineeringStress
:EngineeringStress rdf:type owl:NamedIndividual ,
                            :SeriesType ;
                   rdfs:comment "Represents engineering stress." .


###  http://www.semanticweb.org/ecazares3/ontologies/DynaMat_SHPB#GaugeFactor
:GaugeFactor rdf:type owl:NamedIndividual ,
                      :StrainGaugeFactorType ;
             rdfs:comment "Represents the gauge factor of the strain gauge." .


###  http://www.semanticweb.org/ecazares3/ontologies/DynaMat_SHPB#Incident
:Incident rdf:type owl:NamedIndividual ,
                   :SignalType ;
          rdfs:comment "Indicates the signal from the incident bar." .


###  http://www.semanticweb.org/ecazares3/ontologies/DynaMat_SHPB#MomentumTrapEngaged
:MomentumTrapEngaged rdf:type owl:NamedIndividual ,
                              :MomentumTrap ;
                     rdfs:comment "Indicates that the momentum trap was engaged during the test." .


###  http://www.semanticweb.org/ecazares3/ontologies/DynaMat_SHPB#MomentumTrapNotEngaged
:MomentumTrapNotEngaged rdf:type owl:NamedIndividual ,
                                 :MomentumTrap ;
                        rdfs:comment "Indicates that the momentum trap was not engaged during the test." .


###  http://www.semanticweb.org/ecazares3/ontologies/DynaMat_SHPB#ParticleVelocity
:ParticleVelocity rdf:type owl:NamedIndividual ,
                           :SeriesType ;
                  rdfs:comment "Represents particle velocity at specimen surface." .


###  http://www.semanticweb.org/ecazares3/ontologies/DynaMat_SHPB#PoissonsRatio
:PoissonsRatio rdf:type owl:NamedIndividual ,
                        :MechanicalProperty ;
               rdfs:comment "The ratio of transverse strain to axial strain in the elastic range." .


###  http://www.semanticweb.org/ecazares3/ontologies/DynaMat_SHPB#PulseTest
:PulseTest rdf:type owl:NamedIndividual ,
                    :TestType ;
           rdfs:comment "A calibration test involving pulse evaluation without a specimen." .


###  http://www.semanticweb.org/ecazares3/ontologies/DynaMat_SHPB#Reflected
:Reflected rdf:type owl:NamedIndividual ,
                    :SignalType ;
           rdfs:comment "Indicates the signal reflected within the incident bar." .


###  http://www.semanticweb.org/ecazares3/ontologies/DynaMat_SHPB#Resistance
:Resistance rdf:type owl:NamedIndividual ,
                     :StrainGaugeFactorType ;
            rdfs:comment "Represents the resistance of the strain gauge in ohms." .


###  http://www.semanticweb.org/ecazares3/ontologies/DynaMat_SHPB#SpecimenTest
:SpecimenTest rdf:type owl:NamedIndividual ,
                       :TestType ;
              rdfs:comment "A test involving a specimen to evaluate its mechanical behavior." .


###  http://www.semanticweb.org/ecazares3/ontologies/DynaMat_SHPB#StrainEnergy
:StrainEnergy rdf:type owl:NamedIndividual ,
                       :SeriesType ;
              rdfs:comment "Represents strain energy." .


###  http://www.semanticweb.org/ecazares3/ontologies/DynaMat_SHPB#Transmitted
:Transmitted rdf:type owl:NamedIndividual ,
                      :SignalType ;
             rdfs:comment "Indicates the signal from the transmitted bar." .


###  http://www.semanticweb.org/ecazares3/ontologies/DynaMat_SHPB#TrueStrain
:TrueStrain rdf:type owl:NamedIndividual ,
                     :SeriesType ;
            rdfs:comment "Represents true strain." .


###  http://www.semanticweb.org/ecazares3/ontologies/DynaMat_SHPB#TrueStress
:TrueStress rdf:type owl:NamedIndividual ,
                     :SeriesType ;
            rdfs:comment "Represents true stress." .


###  http://www.semanticweb.org/ecazares3/ontologies/DynaMat_SHPB#WaveSpeed
:WaveSpeed rdf:type owl:NamedIndividual ,
                    :MechanicalProperty ;
           rdfs:comment "Speed of stress waves through the material during testing." .


#################################################################
#    Annotations
#################################################################

:hasDataAcquisitionRate rdfs:comment "Specifies the date the data acquisition rate." .


###  Generated by the OWL API (version 4.5.29.2024-05-13T12:11:03Z) https://github.com/owlcs/owlapi
